theory/x64DecodeProp1.thy
@@ -7,20 +7,7 @@ begin
 
 declare if_split_asm [split]
 declare Let_def [simp]
-declare x64_decode_op_not_rex_def [simp]
-declare x64_decode_op_0x66_def [simp]
-declare x64_decode_op_0x0f_def [simp]
 declare x64_decode_op_0x81_def [simp]
-
-lemma x64_decode_sz_gt_0: "x64_decode pc l = Some (sz, ins) \<Longrightarrow> 0 < sz"
-  apply (simp add: x64_decode_def nth_error_def;
-      (erule case_option_eq_NE; simp?)+)
-  done
-
-declare x64_decode_op_not_rex_def [simp del]
-declare x64_decode_op_0x66_def [simp del]
-declare x64_decode_op_0x0f_def [simp del]
-declare x64_decode_op_0x81_def [simp del]
 
 fun x64_bin_update ::"nat \<Rightarrow> x64_bin \<Rightarrow> nat \<Rightarrow> u8 list \<Rightarrow> x64_bin " where
   "x64_bin_update 0 l _ _ = l" |
@@ -30,12 +17,15 @@ fun x64_bin_update ::"nat \<Rightarrow> x64_bin \<Rightarrow> nat \<Rightarrow> 
   x#xs \<Rightarrow> x64_bin_update n (l[pc := x]) (pc+1) xs
 )"
 
-lemma x64_bin_update_nth_other: "(xpc1 + sz1 \<le> xpc \<or> xpc+sz \<le> xpc1) \<Longrightarrow> xpc1 < length l \<Longrightarrow>
-  sz = (length l1) \<Longrightarrow> 0 < sz1 \<Longrightarrow> 
+lemma x64_bin_update_nth_other: "(xpc1 < xpc \<or> xpc+sz \<le> xpc1) \<Longrightarrow> xpc1 < length l \<Longrightarrow>
+  sz = (length l1) \<Longrightarrow> 
   (x64_bin_update (length l1) l xpc l1)!xpc1 = l!xpc1"
-  apply (induction l1 arbitrary: xpc sz xpc1 sz1 l ; simp)
-  subgoal for a al xpc sz xpc1 sz1 l
-    by (smt (verit, ccfv_threshold) add.commute add_Suc_right leD length_list_update less_add_same_cancel2 list.size(3) not_less_eq_eq nth_list_update_neq x64_bin_update.simps(1) zero_less_Suc)
+  apply (induction l1 arbitrary: xpc sz xpc1 l ; simp)
+  subgoal for a al xpc sz xpc1 l
+    using add.commute add_Suc_right leD length_list_update less_add_same_cancel2 list.size(3)
+      not_less_eq_eq nth_list_update_neq x64_bin_update.simps(1) zero_less_Suc
+    using add_Suc less_SucI less_add_Suc1 by fastforce
+
   done
 
 lemma x64_bin_update_length_eq: "x64_bin_update (length l1) l xpc l1 = l2 \<Longrightarrow> length l = length l2"
@@ -44,18 +34,21 @@ lemma x64_bin_update_length_eq: "x64_bin_update (length l1) l xpc l1 = l2 \<Long
     by auto 
   done
 
-lemma x64_bin_update_nth_error_other: "(xpc1 + sz1 \<le> xpc \<or> xpc+sz \<le> xpc1) \<Longrightarrow> 
-  sz = (length l1) \<Longrightarrow> 0 < sz1 \<Longrightarrow> 
+lemma x64_bin_update_nth_error_other: "
+   x64_bin_update sz l xpc l1 = l2 \<Longrightarrow>
+(xpc1 < xpc \<or> xpc+sz \<le> xpc1) \<Longrightarrow>
+  sz = (length l1) \<Longrightarrow>
   nth_error l xpc1 = Some v \<Longrightarrow> 
-  nth_error (x64_bin_update (length l1) l xpc l1) xpc1 = Some v"
+  nth_error l2 xpc1 = Some v"
   apply (subgoal_tac "length (x64_bin_update (length l1) l xpc l1) = length l")
    prefer 2
   subgoal using x64_bin_update_length_eq
     by metis
   apply (simp add: nth_error_def)
   apply (cases "length l \<le> xpc1"; simp)
-  apply (erule subst [of _v])
-  apply (rule x64_bin_update_nth_other [of xpc1 sz1 xpc sz]; simp?)
+  apply (erule subst [of _ v])
+  apply (erule subst [of _ l2])
+  apply (rule x64_bin_update_nth_other [of xpc1 xpc sz]; simp?)
   done
 
 lemma x64_decode_op_0x66_jcc_false: "x64_decode_op_0x66 xpc l = Some (length u8_list, Pjcc cond d0) \<Longrightarrow> False"
@@ -63,393 +56,1604 @@ lemma x64_decode_op_0x66_jcc_false: "x64_decode_op_0x66 xpc l = Some (length u8_
   apply (erule case_option_eq_NE; simp?)+
   done
 
-lemma x64_decode_op_0x66_jcc_other: "xpc1 + sz1 \<le> xpc \<or> xpc + length u8_list \<le> xpc1 \<Longrightarrow>
-    x64_decode_op_0x0f xpc l = Some (length u8_list, Pjcc cond d0) \<Longrightarrow>
-    x64_decode_op_0x66 xpc1 l = Some (sz1, ins1) \<Longrightarrow>
-    x64_decode_op_0x66 xpc1 (x64_bin_update (length u8_list) l xpc u8_list) = Some (sz1, ins1)"
-  apply (simp add: x64_decode_op_0x0f_def x64_decode_op_0x66_def)
-  apply (erule case_option_eq_NE; simp?)
-  subgoal for op
-    apply (erule case_option_eq_NE; simp?)+
-    done
-  subgoal for op
-    apply (erule case_option_eq_NE; simp?)+
-    done
-  subgoal for op
-    apply (erule case_option_eq_NE; simp?)+
-    subgoal for h1 i1 reg i2 imm i3 dst i4
-      apply (erule conjE)+
-      apply (subgoal_tac "nth_error (x64_bin_update (length u8_list) l xpc u8_list) (Suc xpc1) = Some 193")
-      subgoal
-        apply simp
-        apply (subgoal_tac "nth_error (x64_bin_update (length u8_list) l xpc u8_list) (Suc (Suc xpc1)) = Some reg", simp)
-        subgoal
-          apply (subgoal_tac "nth_error (x64_bin_update (length u8_list) l xpc u8_list) (xpc1 + 3) = Some imm", simp)
-          apply (rule x64_bin_update_nth_error_other [of _ 1]; simp?)
-          apply auto
-          done
-        apply (rule x64_bin_update_nth_error_other [of _ 1]; simp?)
-        apply auto
-        done
-      apply (rule x64_bin_update_nth_error_other [of _ 1]; simp?)
-      apply auto
-      done
-    subgoal for h1 i1 reg 
-      apply (erule case_option_eq_NE; simp?)+
-      subgoal for i2 dst i3 i1a i4 i2a imm
-        apply (subgoal_tac "nth_error (x64_bin_update (length u8_list) l xpc u8_list) (Suc xpc1) = Some 129")
-        subgoal
-          apply simp
-          apply (subgoal_tac "nth_error (x64_bin_update (length u8_list) l xpc u8_list) (Suc (Suc xpc1)) = Some reg", simp)
-          subgoal
-            apply (subgoal_tac "nth_error (x64_bin_update (length u8_list) l xpc u8_list) (xpc1 + 3) = Some i1a", simp)
-            subgoal
-              apply (subgoal_tac "nth_error (x64_bin_update (length u8_list) l xpc u8_list) (xpc1 + 4) = Some i2a", simp)
-              apply (rule x64_bin_update_nth_error_other [of _ 1]; simp?)
-              apply auto
-              done
-            apply (rule x64_bin_update_nth_error_other [of _ 1]; simp?)
-            apply auto
-            done
-          apply (rule x64_bin_update_nth_error_other [of _ 1]; simp?)
-          apply auto
-          done
-        apply (rule x64_bin_update_nth_error_other [of _ 1]; simp?)
-        apply auto
-        done
-      done
-    subgoal for h1 i1 reg 
-      apply (erule case_option_eq_NE; simp?)+
-      subgoal for i2 dis i3 src i4 dst
-        apply (subgoal_tac "nth_error (x64_bin_update (length u8_list) l xpc u8_list) (Suc xpc1) = Some 137")
-        subgoal
-          apply simp
-          apply (subgoal_tac "nth_error (x64_bin_update (length u8_list) l xpc u8_list) (Suc (Suc xpc1)) = Some reg", simp)
-          subgoal
-            apply (subgoal_tac "nth_error (x64_bin_update (length u8_list) l xpc u8_list) (xpc1 + 3) = Some dis", simp)
-            subgoal
-              apply (rule x64_bin_update_nth_error_other [of _ 1]; simp?)
-              apply auto
-              done
-            done
-          apply (rule x64_bin_update_nth_error_other [of _ 1]; simp?)
-          apply auto
-          done
-        apply (rule x64_bin_update_nth_error_other [of _ 1]; simp?)
-        apply auto
-        done
-      done
-    subgoal for h1
-      apply (erule case_option_eq_NE; simp?)+
-      subgoal for i1 opa i2 reg i3 imm i4 dst
-        apply (subgoal_tac "nth_error (x64_bin_update (length u8_list) l xpc u8_list) (Suc xpc1) = Some h1")
-        subgoal
-          apply simp
-          apply (subgoal_tac "nth_error (x64_bin_update (length u8_list) l xpc u8_list) (Suc (Suc xpc1)) = Some 193", simp)
-          subgoal
-            apply (subgoal_tac "nth_error (x64_bin_update (length u8_list) l xpc u8_list) (xpc1 + 3) = Some reg", simp)
-            subgoal
-              apply (subgoal_tac "nth_error (x64_bin_update (length u8_list) l xpc u8_list) (xpc1 + 4) = Some imm", simp)
-              apply (rule x64_bin_update_nth_error_other [of _ 1]; simp?)
-              apply auto
-              done
-            subgoal
-              apply (rule x64_bin_update_nth_error_other [of _ 1]; simp?)
-              apply auto
-              done
-            done
-          apply (rule x64_bin_update_nth_error_other [of _ 1]; simp?)
-          apply auto
-          done
-        apply (rule x64_bin_update_nth_error_other [of _ 1]; simp?)
-        apply auto
-        done
-      subgoal for i1 opa i2 reg
-        apply (erule case_option_eq_NE; simp?)+
-        subgoal for i3 dst i4 i1a i2a imm
-        apply (subgoal_tac "nth_error (x64_bin_update (length u8_list) l xpc u8_list) (Suc xpc1) = Some h1")
-        subgoal
-          apply simp
-          apply (subgoal_tac "nth_error (x64_bin_update (length u8_list) l xpc u8_list) (Suc (Suc xpc1)) = Some 129", simp)
-          subgoal
-            apply (subgoal_tac "nth_error (x64_bin_update (length u8_list) l xpc u8_list) (xpc1 + 3) = Some reg", simp)
-            subgoal
-              apply (subgoal_tac "nth_error (x64_bin_update (length u8_list) l xpc u8_list) (xpc1 + 4) = Some i1a", simp)
-              subgoal
-                apply (subgoal_tac "nth_error (x64_bin_update (length u8_list) l xpc u8_list) (xpc1 + 5) = Some i2a", simp)
-                apply (rule x64_bin_update_nth_error_other [of _ 1]; simp?)
-                apply auto
-                done
-              apply (rule x64_bin_update_nth_error_other [of _ 1]; simp?)
-              apply auto
-              done
-            subgoal
-              apply (rule x64_bin_update_nth_error_other [of _ 1]; simp?)
-              apply auto
-              done
-            done
-          apply (rule x64_bin_update_nth_error_other [of _ 1]; simp?)
-          apply auto
-          done
-        apply (rule x64_bin_update_nth_error_other [of _ 1]; simp?)
-        apply auto
-        done
-      done
-      subgoal for i1 opa i2 reg
-        apply (erule case_option_eq_NE; simp?)+
-        subgoal for i3 dis i4 src dst
-        apply (subgoal_tac "nth_error (x64_bin_update (length u8_list) l xpc u8_list) (Suc xpc1) = Some h1")
-        subgoal
-          apply simp
-          apply (subgoal_tac "nth_error (x64_bin_update (length u8_list) l xpc u8_list) (Suc (Suc xpc1)) = Some 137", simp)
-          subgoal
-            apply (subgoal_tac "nth_error (x64_bin_update (length u8_list) l xpc u8_list) (xpc1 + 3) = Some reg", simp)
-            subgoal
-              apply (subgoal_tac "nth_error (x64_bin_update (length u8_list) l xpc u8_list) (xpc1 + 4) = Some dis", simp)
-              apply (rule x64_bin_update_nth_error_other [of _ 1]; simp?)
-              apply auto
-              done
-            subgoal
-              apply (rule x64_bin_update_nth_error_other [of _ 1]; simp?)
-              apply auto
-              done
-            done
-          apply (rule x64_bin_update_nth_error_other [of _ 1]; simp?)
-          apply auto
-          done
-        apply (rule x64_bin_update_nth_error_other [of _ 1]; simp?)
-        apply auto
-        done
-      done
-    done
-  done
+lemma bitfield_extract_3_5_10_neq_233: "bitfield_extract 3 5 (a1::u8) = 10 \<Longrightarrow> a1 \<noteq> 233"
+  apply (simp add: bitfield_extract_def)
+  apply (simp add: bit_eq_iff)
+  apply (drule_tac x= "2" in spec)
+  apply (simp add: bit_simps)
+  apply (rule_tac x= "5" in exI)
+  apply simp
   done
 
-lemma x64_decode_op_0x0f_jcc_other: "xpc1 + sz1 \<le> xpc \<or> xpc + length u8_list \<le> xpc1 \<Longrightarrow>
-    x64_decode_op_0x0f xpc l = Some (length u8_list, Pjcc cond d0) \<Longrightarrow>
-    x64_decode_op_0x0f xpc1 l = Some (sz1, ins1) \<Longrightarrow>
-      x64_decode_op_0x0f xpc1 (x64_bin_update (length u8_list) l xpc u8_list) = Some (sz1, ins1)"
-  apply (simp add: x64_decode_op_0x0f_def x64_decode_op_0x66_def)
-  apply (erule case_option_eq_NE; simp?)
-  subgoal for op
-    apply (erule case_option_eq_NE; simp?)+
+lemma bitfield_extract_3_5_10_neq_232: "bitfield_extract 3 5 (a1::u8) = 10 \<Longrightarrow> a1 \<noteq> 232"
+  apply (simp add: bitfield_extract_def)
+  apply (simp add: bit_eq_iff)
+  apply (drule_tac x= "2" in spec)
+  apply (simp add: bit_simps)
+  apply (rule_tac x= "5" in exI)
+  apply simp
+  done
+
+lemma bitfield_extract_3_5_11_neq_232: "bitfield_extract 3 5 (a1::u8) = 11 \<Longrightarrow>a1 \<noteq> 232"
+  apply (simp add: bitfield_extract_def)
+  apply (simp add: bit_eq_iff)
+  apply (drule_tac x= "2" in spec)
+  apply (simp add: bit_simps)
+  apply (rule_tac x= "5" in exI)
+  apply simp
+  done
+
+lemma bitfield_extract_3_5_11_neq_233: "bitfield_extract 3 5 (a1::u8) = 11 \<Longrightarrow>a1 \<noteq> 233"
+  apply (simp add: bitfield_extract_def)
+  apply (simp add: bit_eq_iff)
+  apply (drule_tac x= "2" in spec)
+  apply (simp add: bit_simps)
+  apply (rule_tac x= "5" in exI)
+  apply simp
+  done
+
+declare if_split_asm [split del]
+
+
+lemma ifE:
+  assumes c: "(if Q then x else y) = R"
+  obtains
+    "Q = True \<and> x = R" 
+  | "Q = False \<and> y = R"
+  using c by argo
+
+declare add_2_eq_Suc [simp del]
+declare add_2_eq_Suc' [simp del]
+declare One_nat_def [simp del]
+
+lemma x64_encode_x64_decode_other_x64_decode_op_0x66_0: "
+  xpc1 + sz1 \<le> xpc \<or> xpc + 6 \<le> xpc1 \<Longrightarrow> length u8_list = 6 \<Longrightarrow> sz = 6 \<Longrightarrow>
+  x64_bin_update 6 l xpc u8_list = l1 \<Longrightarrow> nth_error l xpc1 = Some 102 \<Longrightarrow> h = 102 \<Longrightarrow>
+  x64_decode_op_0x66 xpc1 l = Some (sz1, ins1) \<Longrightarrow> xpc1 < xpc \<or> xpc + 6 \<le> xpc1"
+  apply (simp add: x64_decode_op_0x66_def)
+  apply ((erule case_option_eq_NE; simp?) | (erule ifE; erule conjE; simp))+
+  subgoal for h1 reg imm dst
+    by linarith
+  subgoal for h1 reg
+    apply ((erule case_option_eq_NE; simp?) | (erule ifE; erule conjE; simp))+
+    subgoal for dst i1 i2 imm
+      by linarith
+    apply ((erule case_option_eq_NE; simp?) | (erule ifE; erule conjE; simp))+
+    subgoal
+      by linarith
     done
-  subgoal for op
-    apply (erule case_option_eq_NE; simp?)+
-    done
-  subgoal for op
-    apply (erule case_option_eq_NE; simp?)+
-    subgoal for opa i1 i2 i3 i4
-      apply (erule conjE)+
-      apply (subgoal_tac "nth_error (x64_bin_update (length u8_list) l xpc u8_list) (Suc xpc1) = Some 49")
-      subgoal
-        apply simp
-        done
-        apply (rule x64_bin_update_nth_error_other [of _ 1]; simp?)
-        apply auto
-        done
-    subgoal for opa
-      apply (erule case_option_eq_NE; simp?)+
-      subgoal for i1 dst i2 i3 i4
-      apply (subgoal_tac "nth_error (x64_bin_update (length u8_list) l xpc u8_list) (Suc xpc1) = Some opa")
-      subgoal
-        apply simp
-        done
-        apply (rule x64_bin_update_nth_error_other [of _ 1]; simp?)
-        apply auto
-        done
-      done
-    subgoal for opa
-      apply (erule case_option_eq_NE; simp?)+
-      subgoal for i1 reg i2 t i3 src i4 dst
-        apply (subgoal_tac "nth_error (x64_bin_update (length u8_list) l xpc u8_list) (Suc xpc1) = Some opa", simp)
-        subgoal
-          apply (subgoal_tac "nth_error (x64_bin_update (length u8_list) l xpc u8_list) (Suc (Suc xpc1)) = Some reg", simp)
-          apply (rule x64_bin_update_nth_error_other [of _ 1]; simp?)
-          apply auto
-          done
-        apply (rule x64_bin_update_nth_error_other [of _ 1]; simp?)
-        apply auto
-        done
-      done
-    subgoal for opa
-      apply (erule case_option_eq_NE; simp?)+
-      subgoal for i1 i1a i2 i2a i3 i3a i4 i4a da t
-        apply (subgoal_tac "nth_error (x64_bin_update (length u8_list) l xpc u8_list) (Suc xpc1) = Some opa", simp)
-        subgoal
-          apply (subgoal_tac "nth_error (x64_bin_update (length u8_list) l xpc u8_list) (Suc (Suc xpc1)) = Some i1a", simp)
-          subgoal
-            apply (subgoal_tac "nth_error (x64_bin_update (length u8_list) l xpc u8_list) (xpc1 + 3) = Some i2a", simp)
-            subgoal
-              apply (subgoal_tac "nth_error (x64_bin_update (length u8_list) l xpc u8_list) (xpc1 + 4) = Some i3a", simp)
-              subgoal
-                apply (subgoal_tac "nth_error (x64_bin_update (length u8_list) l xpc u8_list) (xpc1 + 5) = Some i4a", simp)
-                apply (rule x64_bin_update_nth_error_other [of _ 1]; simp?)
-                apply auto
-                done
-              apply (rule x64_bin_update_nth_error_other [of _ 1]; simp?)
-              apply auto
-              done
-            apply (rule x64_bin_update_nth_error_other [of _ 1]; simp?)
-            apply auto
-            done
-          apply (rule x64_bin_update_nth_error_other [of _ 1]; simp?)
-          apply auto
-          done
-        apply (rule x64_bin_update_nth_error_other [of _ 1]; simp?)
-        apply auto
-        done
-      done
+  subgoal
+    apply ((erule case_option_eq_NE; simp?) | (erule ifE; erule conjE; simp))+
+    subgoal
+      by linarith
+    apply ((erule case_option_eq_NE; simp?) | (erule ifE; erule conjE; simp))+
+    subgoal
+      by linarith
+    subgoal
+    apply ((erule case_option_eq_NE; simp?) | (erule ifE; erule conjE; simp))+
+      by linarith
     done
   done
 
-lemma x64_decode_op_not_rex_jcc_other: "xpc1 + sz1 \<le> xpc \<or> xpc + length u8_list \<le> xpc1 \<Longrightarrow>
-    x64_decode_op_0x0f xpc l = Some (length u8_list, Pjcc cond d0) \<Longrightarrow>
-    x64_decode_op_not_rex a1 xpc1 l = Some (sz1, ins1) \<Longrightarrow>
-    x64_decode_op_not_rex a1 xpc1 (x64_bin_update (length u8_list) l xpc u8_list) = Some (sz1, ins1)"
-  apply (simp add: x64_decode_op_0x0f_def x64_decode_op_not_rex_def)
-  apply (erule case_option_eq_NE; simp?)
-  subgoal for op
-    apply (erule case_option_eq_NE; simp?)+
+lemma x64_encode_x64_decode_other_x64_decode_op_0x66_1: "
+  xpc1 + sz1 \<le> xpc \<or> xpc + 6 \<le> xpc1 \<Longrightarrow> length u8_list = 6 \<Longrightarrow> sz = 6 \<Longrightarrow>
+  x64_bin_update 6 l xpc u8_list = l1 \<Longrightarrow> nth_error l xpc1 = Some 102 \<Longrightarrow> h = 102 \<Longrightarrow>
+  x64_decode_op_0x66 xpc1 l = Some (sz1, ins1) \<Longrightarrow> x64_decode_op_0x66 xpc1 l1 = Some (sz1, ins1)"
+  apply (simp add: x64_decode_op_0x66_def)
+  apply ((erule case_option_eq_NE; simp?) | (erule ifE; erule conjE; simp))+
+  subgoal for h1 reg imm dst
+    apply (subst x64_bin_update_nth_error_other [of 6 l xpc u8_list l1 "xpc1+1" h1]; simp?; linarith?)
+    apply (subst x64_bin_update_nth_error_other [of 6 l xpc u8_list l1 "xpc1+2" reg]; simp?; linarith?)
+    apply (subst x64_bin_update_nth_error_other [of 6 l xpc u8_list l1 "xpc1+3" imm]; simp?; linarith?)
     done
-  subgoal for op
-    apply (erule case_option_eq_NE; simp?)+
+
+  apply ((erule case_option_eq_NE; simp?) | (erule ifE; erule conjE; simp))+
+  subgoal for h1 reg dst i1 i2 imm
+    apply (subst x64_bin_update_nth_error_other [of 6 l xpc u8_list l1 "xpc1+1" h1]; simp?; linarith?)
+    apply (subst x64_bin_update_nth_error_other [of 6 l xpc u8_list l1 "xpc1+2" reg]; simp?; linarith?)
+    apply (subst x64_bin_update_nth_error_other [of 6 l xpc u8_list l1 "xpc1+3" i1]; simp?; linarith?)
+    apply (subst x64_bin_update_nth_error_other [of 6 l xpc u8_list l1 "xpc1+4" i2]; simp?; linarith?)
     done
+  apply ((erule case_option_eq_NE; simp?) | (erule ifE; erule conjE; simp))+
+  subgoal for h1 reg dis src dst
+    apply (subst x64_bin_update_nth_error_other [of 6 l xpc u8_list l1 "xpc1+1" h1]; simp?; linarith?)
+    apply (subst x64_bin_update_nth_error_other [of 6 l xpc u8_list l1 "xpc1+2" reg]; simp?; linarith?)
+    apply (subst x64_bin_update_nth_error_other [of 6 l xpc u8_list l1 "xpc1+3" dis]; simp?; linarith?)
+    done
+  apply ((erule case_option_eq_NE; simp?) | (erule ifE; erule conjE; simp))+
+  subgoal for h1 op reg imm dst
+    apply (subst x64_bin_update_nth_error_other [of 6 l xpc u8_list l1 "xpc1+1" h1]; simp?; linarith?)
+    apply (subst x64_bin_update_nth_error_other [of 6 l xpc u8_list l1 "xpc1+2" op]; simp?; linarith?)
+    apply (subst x64_bin_update_nth_error_other [of 6 l xpc u8_list l1 "xpc1+3" reg]; simp?; linarith?)
+    apply (subst x64_bin_update_nth_error_other [of 6 l xpc u8_list l1 "xpc1+4" imm]; simp?; linarith?)
+    done
+  apply ((erule case_option_eq_NE; simp?) | (erule ifE; erule conjE; simp))+
+  subgoal for h1 op reg dst i1 i2 imm
+    apply (subst x64_bin_update_nth_error_other [of 6 l xpc u8_list l1 "xpc1+1" h1]; simp?; linarith?)
+    apply (subst x64_bin_update_nth_error_other [of 6 l xpc u8_list l1 "xpc1+2" op]; simp?; linarith?)
+    apply (subst x64_bin_update_nth_error_other [of 6 l xpc u8_list l1 "xpc1+3" reg]; simp?; linarith?)
+    apply (subst x64_bin_update_nth_error_other [of 6 l xpc u8_list l1 "xpc1+4" i1]; simp?; linarith?)
+    apply (subst x64_bin_update_nth_error_other [of 6 l xpc u8_list l1 "xpc1+5" i2]; simp?; linarith?)
+    done
+  apply ((erule case_option_eq_NE; simp?) | (erule ifE; erule conjE; simp))+
+  subgoal for h1 op reg dis src dst
+    apply (subst x64_bin_update_nth_error_other [of 6 l xpc u8_list l1 "xpc1+1" h1]; simp?; linarith?)
+    apply (subst x64_bin_update_nth_error_other [of 6 l xpc u8_list l1 "xpc1+2" op]; simp?; linarith?)
+    apply (subst x64_bin_update_nth_error_other [of 6 l xpc u8_list l1 "xpc1+3" reg]; simp?; linarith?)
+    apply (subst x64_bin_update_nth_error_other [of 6 l xpc u8_list l1 "xpc1+4" dis]; simp?; linarith?)
+    done
+  done
+
+
+
+lemma x64_encode_x64_decode_other_x64_decode_op_0x0f_0: "
+  xpc1 + sz1 \<le> xpc \<or> xpc + 6 \<le> xpc1 \<Longrightarrow> length u8_list = 6 \<Longrightarrow> sz = 6 \<Longrightarrow>
+  x64_bin_update 6 l xpc u8_list = l1 \<Longrightarrow> nth_error l xpc1 = Some 15 \<Longrightarrow> h = 15 \<Longrightarrow>
+  x64_decode_op_0x0f xpc1 l = Some (sz1, ins1) \<Longrightarrow> xpc1 < xpc \<or> xpc + 6 \<le> xpc1"
+  apply (simp add: x64_decode_op_0x0f_def)
+  apply ((erule case_option_eq_NE; simp?) | (erule ifE; erule conjE; simp))+
   subgoal for op
-    apply (erule case_option_eq_NE; simp?)+
-    subgoal for dst i1 i2 i3 i4
-      apply (erule conjE)+
-      apply (subgoal_tac "nth_error (x64_bin_update (length u8_list) l xpc u8_list) (Suc xpc1) = Some 49")
-      subgoal
-        apply simp
-        done
-        apply (rule x64_bin_update_nth_error_other [of _ 1]; simp?)
-        apply auto
-        done
-    subgoal for opa
-      apply (erule case_option_eq_NE; simp?)+
-      subgoal for i1 dst i2 i3 i4
-      apply (subgoal_tac "nth_error (x64_bin_update (length u8_list) l xpc u8_list) (Suc xpc1) = Some opa")
-      subgoal
-        apply simp
-        done
-        apply (rule x64_bin_update_nth_error_other [of _ 1]; simp?)
-        apply auto
-        done
-      done
-    subgoal for opa
-      apply (erule case_option_eq_NE; simp?)+
-      subgoal for i1 reg i2 t i3 src i4 dst
-        apply (subgoal_tac "nth_error (x64_bin_update (length u8_list) l xpc u8_list) (Suc xpc1) = Some opa", simp)
-        subgoal
-          apply (subgoal_tac "nth_error (x64_bin_update (length u8_list) l xpc u8_list) (Suc (Suc xpc1)) = Some reg", simp)
-          apply (rule x64_bin_update_nth_error_other [of _ 1]; simp?)
-          apply auto
-          done
-        apply (rule x64_bin_update_nth_error_other [of _ 1]; simp?)
-        apply auto
-        done
-      done
-    subgoal for opa
-      apply (erule case_option_eq_NE; simp?)+
-      subgoal for i1 i1a i2 i2a i3 i3a i4 i4a da t
-        apply (subgoal_tac "nth_error (x64_bin_update (length u8_list) l xpc u8_list) (Suc xpc1) = Some opa", simp)
-        subgoal
-          apply (subgoal_tac "nth_error (x64_bin_update (length u8_list) l xpc u8_list) (Suc (Suc xpc1)) = Some i1a", simp)
-          subgoal
-            apply (subgoal_tac "nth_error (x64_bin_update (length u8_list) l xpc u8_list) (xpc1 + 3) = Some i2a", simp)
-            subgoal
-              apply (subgoal_tac "nth_error (x64_bin_update (length u8_list) l xpc u8_list) (xpc1 + 4) = Some i3a", simp)
-              subgoal
-                apply (subgoal_tac "nth_error (x64_bin_update (length u8_list) l xpc u8_list) (xpc1 + 5) = Some i4a", simp)
-                apply (rule x64_bin_update_nth_error_other [of _ 1]; simp?)
-                apply auto
-                done
-              apply (rule x64_bin_update_nth_error_other [of _ 1]; simp?)
-              apply auto
-              done
-            apply (rule x64_bin_update_nth_error_other [of _ 1]; simp?)
-            apply auto
-            done
-          apply (rule x64_bin_update_nth_error_other [of _ 1]; simp?)
-          apply auto
-          done
-        apply (rule x64_bin_update_nth_error_other [of _ 1]; simp?)
-        apply auto
-        done
-      done
+    by linarith
+  apply ((erule case_option_eq_NE; simp?) | (erule ifE; erule conjE; simp))+
+  subgoal
+    by linarith
+
+    apply ((erule case_option_eq_NE; simp?) | (erule ifE; erule conjE; simp))+
+    subgoal
+      by linarith
+    apply ((erule case_option_eq_NE; simp?) | (erule ifE; erule conjE; simp))+
+    subgoal
+      by linarith
+    done
+
+lemma x64_encode_x64_decode_other_x64_decode_op_0x0f_1: "
+  xpc1 + sz1 \<le> xpc \<or> xpc + 6 \<le> xpc1 \<Longrightarrow> length u8_list = 6 \<Longrightarrow> sz = 6 \<Longrightarrow>
+  x64_bin_update 6 l xpc u8_list = l1 \<Longrightarrow> nth_error l xpc1 = Some 15 \<Longrightarrow> h = 15 \<Longrightarrow> 
+  x64_decode_op_0x0f xpc1 l = Some (sz1, ins1) \<Longrightarrow> x64_decode_op_0x0f xpc1 l1 = Some (sz1, ins1)"
+  apply (simp add: x64_decode_op_0x0f_def)
+  apply ((erule case_option_eq_NE; simp?) | (erule ifE; erule conjE; simp))+
+  subgoal for op
+    apply (subst x64_bin_update_nth_error_other [of 6 l xpc u8_list l1 "xpc1+1" op]; simp?; linarith?)
+    done
+
+  apply ((erule case_option_eq_NE; simp?) | (erule ifE; erule conjE; simp))+
+  subgoal for op dst
+    apply (subst x64_bin_update_nth_error_other [of 6 l xpc u8_list l1 "xpc1+1" op]; simp?; linarith?)
+    done
+  apply ((erule case_option_eq_NE; simp?) | (erule ifE; erule conjE; simp))+
+  subgoal for op reg t src dst
+    apply (subst x64_bin_update_nth_error_other [of 6 l xpc u8_list l1 "xpc1+1" op]; simp?; linarith?)
+    apply (subst x64_bin_update_nth_error_other [of 6 l xpc u8_list l1 "xpc1+2" reg]; simp?; linarith?)
+    done
+  apply ((erule case_option_eq_NE; simp?) | (erule ifE; erule conjE; simp))+
+  subgoal for op i1 i2 i3 i4 d t
+    apply (subst x64_bin_update_nth_error_other [of 6 l xpc u8_list l1 "xpc1+1" op]; simp?; linarith?)
+    apply (subst x64_bin_update_nth_error_other [of 6 l xpc u8_list l1 "xpc1+2" i1]; simp?; linarith?)
+    apply (subst x64_bin_update_nth_error_other [of 6 l xpc u8_list l1 "xpc1+3" i2]; simp?; linarith?)
+    apply (subst x64_bin_update_nth_error_other [of 6 l xpc u8_list l1 "xpc1+4" i3]; simp?; linarith?)
+    apply (subst x64_bin_update_nth_error_other [of 6 l xpc u8_list l1 "xpc1+5" i4]; simp?; linarith?)
+    done
+  done
+
+
+lemma x64_encode_x64_decode_other_x64_decode_op_not_rex_0: "
+  xpc1 + sz1 \<le> xpc \<or> xpc + 6 \<le> xpc1 \<Longrightarrow> length u8_list = 6 \<Longrightarrow>
+  sz = 6 \<Longrightarrow> x64_bin_update 6 l xpc u8_list = l1 \<Longrightarrow> nth_error l xpc1 = Some h \<Longrightarrow> h \<noteq> 144 \<Longrightarrow>
+  h \<noteq> 153 \<Longrightarrow> h \<noteq> 195 \<Longrightarrow> h \<noteq> 102 \<Longrightarrow> h \<noteq> 15 \<Longrightarrow> bitfield_extract 4 4 h \<noteq> 4 \<Longrightarrow>
+  x64_decode_op_not_rex h xpc1 l = Some (sz1, ins1) \<Longrightarrow> xpc1 < xpc \<or> xpc + 6 \<le> xpc1"
+  apply (simp add: x64_decode_op_not_rex_def)
+  apply ((erule case_option_eq_NE; simp?) | (erule ifE; erule conjE; simp) | linarith)+
+  done
+
+
+lemma x64_encode_x64_decode_other_x64_decode_op_not_rex_1: "
+  xpc1 + sz1 \<le> xpc \<or> xpc + 6 \<le> xpc1 \<Longrightarrow> length u8_list = 6 \<Longrightarrow> sz = 6 \<Longrightarrow>
+    x64_bin_update 6 l xpc u8_list = l1 \<Longrightarrow>
+    nth_error l xpc1 = Some h \<Longrightarrow> h \<noteq> 144 \<Longrightarrow> h \<noteq> 153 \<Longrightarrow> h \<noteq> 195 \<Longrightarrow> h \<noteq> 102 \<Longrightarrow> h \<noteq> 15 \<Longrightarrow>
+  bitfield_extract 4 4 h \<noteq> 4 \<Longrightarrow> x64_decode_op_not_rex h xpc1 l = Some (sz1, ins1) \<Longrightarrow>
+  x64_decode_op_not_rex h xpc1 l1 = Some (sz1, ins1)"
+  apply (simp add: x64_decode_op_not_rex_def)
+  apply ((erule case_option_eq_NE; simp?) | (erule ifE; erule conjE; simp))+
+  subgoal for dst
+    using bitfield_extract_3_5_10_neq_233 by auto
+  apply ((erule case_option_eq_NE; simp?) | (erule ifE; erule conjE; simp))+
+  subgoal for dst
+    using bitfield_extract_3_5_10_neq_233 by auto
+  apply ((erule case_option_eq_NE; simp?) | (erule ifE; erule conjE; simp))+
+  subgoal for i1 i2 i3 i4 d 
+    apply (subst x64_bin_update_nth_error_other [of 6 l xpc u8_list l1 "xpc1+1" i1]; simp?; linarith?)
+    apply (subst x64_bin_update_nth_error_other [of 6 l xpc u8_list l1 "xpc1+2" i2]; simp?; linarith?)
+    apply (subst x64_bin_update_nth_error_other [of 6 l xpc u8_list l1 "xpc1+3" i3]; simp?; linarith?)
+    apply (subst x64_bin_update_nth_error_other [of 6 l xpc u8_list l1 "xpc1+4" i4]; simp?; linarith?)
+    done
+  apply ((erule case_option_eq_NE; simp?) | (erule ifE; erule conjE; simp))+
+  subgoal for i1 i2 i3 i4 d 
+    apply (subst x64_bin_update_nth_error_other [of 6 l xpc u8_list l1 "xpc1+1" i1]; simp?; linarith?)
+    apply (subst x64_bin_update_nth_error_other [of 6 l xpc u8_list l1 "xpc1+2" i2]; simp?; linarith?)
+    apply (subst x64_bin_update_nth_error_other [of 6 l xpc u8_list l1 "xpc1+3" i3]; simp?; linarith?)
+    apply (subst x64_bin_update_nth_error_other [of 6 l xpc u8_list l1 "xpc1+4" i4]; simp?; linarith?)
+    done
+  apply ((erule case_option_eq_NE; simp?) | (erule ifE; erule conjE; simp))+
+  subgoal for reg src dst
+    apply (subst x64_bin_update_nth_error_other [of 6 l xpc u8_list l1 "xpc1+1" reg]; simp?; linarith?)
+    done
+  apply ((erule case_option_eq_NE; simp?) | (erule ifE; erule conjE; simp))+
+  subgoal for reg dis src dst
+    apply (subst x64_bin_update_nth_error_other [of 6 l xpc u8_list l1 "xpc1+1" reg]; simp?; linarith?)
+    apply (subst x64_bin_update_nth_error_other [of 6 l xpc u8_list l1 "xpc1+2" dis]; simp?; linarith?)
+    done
+  apply ((erule case_option_eq_NE; simp?) | (erule ifE; erule conjE; simp))+
+  subgoal for reg d1 d2 d3 d4 dis src dst
+    apply (subst x64_bin_update_nth_error_other [of 6 l xpc u8_list l1 "xpc1+1" reg]; simp?; linarith?)
+    apply (subst x64_bin_update_nth_error_other [of 6 l xpc u8_list l1 "xpc1+2" d1]; simp?; linarith?)
+    apply (subst x64_bin_update_nth_error_other [of 6 l xpc u8_list l1 "xpc1+3" d2]; simp?; linarith?)
+    apply (subst x64_bin_update_nth_error_other [of 6 l xpc u8_list l1 "xpc1+4" d3]; simp?; linarith?)
+    apply (subst x64_bin_update_nth_error_other [of 6 l xpc u8_list l1 "xpc1+5" d4]; simp?; linarith?)
+    done
+  apply ((erule case_option_eq_NE; simp?) | (erule ifE; erule conjE; simp))+
+  subgoal for reg src dst
+    apply (subst x64_bin_update_nth_error_other [of 6 l xpc u8_list l1 "xpc1+1" reg]; simp?; linarith?)
+    done
+  apply ((erule case_option_eq_NE; simp?) | (erule ifE; erule conjE; simp))+
+  subgoal for reg dst
+    apply (subst x64_bin_update_nth_error_other [of 6 l xpc u8_list l1 "xpc1+1" reg]; simp?; linarith?)
+    done
+  apply ((erule case_option_eq_NE; simp?) | (erule ifE; erule conjE; simp))+
+  subgoal for reg dst
+    apply (subst x64_bin_update_nth_error_other [of 6 l xpc u8_list l1 "xpc1+1" reg]; simp?; linarith?)
+    done
+  apply ((erule case_option_eq_NE; simp?) | (erule ifE; erule conjE; simp))+
+  subgoal for reg dst
+    apply (subst x64_bin_update_nth_error_other [of 6 l xpc u8_list l1 "xpc1+1" reg]; simp?; linarith?)
+    done
+  apply ((erule case_option_eq_NE; simp?) | (erule ifE; erule conjE; simp))+
+  subgoal for reg dst
+    apply (subst x64_bin_update_nth_error_other [of 6 l xpc u8_list l1 "xpc1+1" reg]; simp?; linarith?)
+    done
+  apply ((erule case_option_eq_NE; simp?) | (erule ifE; erule conjE; simp))+
+  subgoal for reg dst
+    apply (subst x64_bin_update_nth_error_other [of 6 l xpc u8_list l1 "xpc1+1" reg]; simp?; linarith?)
+    done
+  apply ((erule case_option_eq_NE; simp?) | (erule ifE; erule conjE; simp))+
+  subgoal for reg i1 i2 i3 i4 dst imm
+    apply (subst x64_bin_update_nth_error_other [of 6 l xpc u8_list l1 "xpc1+1" reg]; simp?; linarith?)
+    apply (subst x64_bin_update_nth_error_other [of 6 l xpc u8_list l1 "xpc1+2" i1]; simp?; linarith?)
+    apply (subst x64_bin_update_nth_error_other [of 6 l xpc u8_list l1 "xpc1+3" i2]; simp?; linarith?)
+    apply (subst x64_bin_update_nth_error_other [of 6 l xpc u8_list l1 "xpc1+4" i3]; simp?; linarith?)
+    apply (subst x64_bin_update_nth_error_other [of 6 l xpc u8_list l1 "xpc1+5" i4]; simp?; linarith?)
+    done
+  apply ((erule case_option_eq_NE; simp?) | (erule ifE; erule conjE; simp))+
+  subgoal for reg src dst
+    apply (subst x64_bin_update_nth_error_other [of 6 l xpc u8_list l1 "xpc1+1" reg]; simp?; linarith?)
+    done
+  apply ((erule case_option_eq_NE; simp?) | (erule ifE; erule conjE; simp))+
+  subgoal for reg src dst
+    apply (subst x64_bin_update_nth_error_other [of 6 l xpc u8_list l1 "xpc1+1" reg]; simp?; linarith?)
+    done
+  apply ((erule case_option_eq_NE; simp?) | (erule ifE; erule conjE; simp))+
+  subgoal for reg src dst
+    apply (subst x64_bin_update_nth_error_other [of 6 l xpc u8_list l1 "xpc1+1" reg]; simp?; linarith?)
+    done
+  apply ((erule case_option_eq_NE; simp?) | (erule ifE; erule conjE; simp))+
+  subgoal for reg src dst
+    apply (subst x64_bin_update_nth_error_other [of 6 l xpc u8_list l1 "xpc1+1" reg]; simp?; linarith?)
+    done
+  apply ((erule case_option_eq_NE; simp?) | (erule ifE; erule conjE; simp))+
+  subgoal for reg dst
+    apply (subst x64_bin_update_nth_error_other [of 6 l xpc u8_list l1 "xpc1+1" reg]; simp?; linarith?)
+    done
+  apply ((erule case_option_eq_NE; simp?) | (erule ifE; erule conjE; simp))+
+  subgoal for reg dst
+    apply (subst x64_bin_update_nth_error_other [of 6 l xpc u8_list l1 "xpc1+1" reg]; simp?; linarith?)
+    done
+  apply ((erule case_option_eq_NE; simp?) | (erule ifE; erule conjE; simp))+
+  subgoal for reg dst
+    apply (subst x64_bin_update_nth_error_other [of 6 l xpc u8_list l1 "xpc1+1" reg]; simp?; linarith?)
+    done
+  apply ((erule case_option_eq_NE; simp?) | (erule ifE; erule conjE; simp))+
+  subgoal for reg dst
+    apply (subst x64_bin_update_nth_error_other [of 6 l xpc u8_list l1 "xpc1+1" reg]; simp?; linarith?)
+    done
+  apply ((erule case_option_eq_NE; simp?) | (erule ifE; erule conjE; simp))+
+  subgoal for reg dst
+    apply (subst x64_bin_update_nth_error_other [of 6 l xpc u8_list l1 "xpc1+1" reg]; simp?; linarith?)
+    done
+  apply ((erule case_option_eq_NE; simp?) | (erule ifE; erule conjE; simp))+
+  subgoal for reg dst
+    apply (subst x64_bin_update_nth_error_other [of 6 l xpc u8_list l1 "xpc1+1" reg]; simp?; linarith?)
+    done
+  apply ((erule case_option_eq_NE; simp?) | (erule ifE; erule conjE; simp))+
+  subgoal for reg i1 i2 i3 i4 dst imm
+    apply (subst x64_bin_update_nth_error_other [of 6 l xpc u8_list l1 "xpc1+1" reg]; simp?; linarith?)
+    apply (subst x64_bin_update_nth_error_other [of 6 l xpc u8_list l1 "xpc1+2" i1]; simp?; linarith?)
+    apply (subst x64_bin_update_nth_error_other [of 6 l xpc u8_list l1 "xpc1+3" i2]; simp?; linarith?)
+    apply (subst x64_bin_update_nth_error_other [of 6 l xpc u8_list l1 "xpc1+4" i3]; simp?; linarith?)
+    apply (subst x64_bin_update_nth_error_other [of 6 l xpc u8_list l1 "xpc1+5" i4]; simp?; linarith?)
+    done
+  apply ((erule case_option_eq_NE; simp?) | (erule ifE; erule conjE; simp))+
+  subgoal for reg imm dst
+    apply (subst x64_bin_update_nth_error_other [of 6 l xpc u8_list l1 "xpc1+1" reg]; simp?; linarith?)
+    apply (subst x64_bin_update_nth_error_other [of 6 l xpc u8_list l1 "xpc1+2" imm]; simp?; linarith?)
+    done
+  apply ((erule case_option_eq_NE; simp?) | (erule ifE; erule conjE; simp))+
+  subgoal for reg imm dst
+    apply (subst x64_bin_update_nth_error_other [of 6 l xpc u8_list l1 "xpc1+1" reg]; simp?; linarith?)
+    apply (subst x64_bin_update_nth_error_other [of 6 l xpc u8_list l1 "xpc1+2" imm]; simp?; linarith?)
+    done
+  apply ((erule case_option_eq_NE; simp?) | (erule ifE; erule conjE; simp))+
+  subgoal for reg imm dst
+    apply (subst x64_bin_update_nth_error_other [of 6 l xpc u8_list l1 "xpc1+1" reg]; simp?; linarith?)
+    apply (subst x64_bin_update_nth_error_other [of 6 l xpc u8_list l1 "xpc1+2" imm]; simp?; linarith?)
+    done
+  apply ((erule case_option_eq_NE; simp?) | (erule ifE; erule conjE; simp))+
+  subgoal for reg dst i1 i2 i3 i4 imm
+    apply (subst x64_bin_update_nth_error_other [of 6 l xpc u8_list l1 "xpc1+1" reg]; simp?; linarith?)
+    apply (subst x64_bin_update_nth_error_other [of 6 l xpc u8_list l1 "xpc1+2" i1]; simp?; linarith?)
+    apply (subst x64_bin_update_nth_error_other [of 6 l xpc u8_list l1 "xpc1+3" i2]; simp?; linarith?)
+    apply (subst x64_bin_update_nth_error_other [of 6 l xpc u8_list l1 "xpc1+4" i3]; simp?; linarith?)
+    apply (subst x64_bin_update_nth_error_other [of 6 l xpc u8_list l1 "xpc1+5" i4]; simp?; linarith?)
+    done
+  apply ((erule case_option_eq_NE; simp?) | (erule ifE; erule conjE; simp))+
+  subgoal for reg dst i1 i2 i3 i4 imm
+    apply (subst x64_bin_update_nth_error_other [of 6 l xpc u8_list l1 "xpc1+1" reg]; simp?; linarith?)
+    apply (subst x64_bin_update_nth_error_other [of 6 l xpc u8_list l1 "xpc1+2" i1]; simp?; linarith?)
+    apply (subst x64_bin_update_nth_error_other [of 6 l xpc u8_list l1 "xpc1+3" i2]; simp?; linarith?)
+    apply (subst x64_bin_update_nth_error_other [of 6 l xpc u8_list l1 "xpc1+4" i3]; simp?; linarith?)
+    apply (subst x64_bin_update_nth_error_other [of 6 l xpc u8_list l1 "xpc1+5" i4]; simp?; linarith?)
+    done
+  apply ((erule case_option_eq_NE; simp?) | (erule ifE; erule conjE; simp))+
+  subgoal for reg dst i1 i2 i3 i4 imm
+    apply (subst x64_bin_update_nth_error_other [of 6 l xpc u8_list l1 "xpc1+1" reg]; simp?; linarith?)
+    apply (subst x64_bin_update_nth_error_other [of 6 l xpc u8_list l1 "xpc1+2" i1]; simp?; linarith?)
+    apply (subst x64_bin_update_nth_error_other [of 6 l xpc u8_list l1 "xpc1+3" i2]; simp?; linarith?)
+    apply (subst x64_bin_update_nth_error_other [of 6 l xpc u8_list l1 "xpc1+4" i3]; simp?; linarith?)
+    apply (subst x64_bin_update_nth_error_other [of 6 l xpc u8_list l1 "xpc1+5" i4]; simp?; linarith?)
+    done
+  apply ((erule case_option_eq_NE; simp?) | (erule ifE; erule conjE; simp))+
+  subgoal for reg dst i1 i2 i3 i4 imm
+    apply (subst x64_bin_update_nth_error_other [of 6 l xpc u8_list l1 "xpc1+1" reg]; simp?; linarith?)
+    apply (subst x64_bin_update_nth_error_other [of 6 l xpc u8_list l1 "xpc1+2" i1]; simp?; linarith?)
+    apply (subst x64_bin_update_nth_error_other [of 6 l xpc u8_list l1 "xpc1+3" i2]; simp?; linarith?)
+    apply (subst x64_bin_update_nth_error_other [of 6 l xpc u8_list l1 "xpc1+4" i3]; simp?; linarith?)
+    apply (subst x64_bin_update_nth_error_other [of 6 l xpc u8_list l1 "xpc1+5" i4]; simp?; linarith?)
+    done
+  apply ((erule case_option_eq_NE; simp?) | (erule ifE; erule conjE; simp))+
+  subgoal for reg dst i1 i2 i3 i4 imm
+    apply (subst x64_bin_update_nth_error_other [of 6 l xpc u8_list l1 "xpc1+1" reg]; simp?; linarith?)
+    apply (subst x64_bin_update_nth_error_other [of 6 l xpc u8_list l1 "xpc1+2" i1]; simp?; linarith?)
+    apply (subst x64_bin_update_nth_error_other [of 6 l xpc u8_list l1 "xpc1+3" i2]; simp?; linarith?)
+    apply (subst x64_bin_update_nth_error_other [of 6 l xpc u8_list l1 "xpc1+4" i3]; simp?; linarith?)
+    apply (subst x64_bin_update_nth_error_other [of 6 l xpc u8_list l1 "xpc1+5" i4]; simp?; linarith?)
+    done
+  apply ((erule case_option_eq_NE; simp?) | (erule ifE; erule conjE; simp))+
+  subgoal for reg dst i1 i2 i3 i4 imm
+    apply (subst x64_bin_update_nth_error_other [of 6 l xpc u8_list l1 "xpc1+1" reg]; simp?; linarith?)
+    apply (subst x64_bin_update_nth_error_other [of 6 l xpc u8_list l1 "xpc1+2" i1]; simp?; linarith?)
+    apply (subst x64_bin_update_nth_error_other [of 6 l xpc u8_list l1 "xpc1+3" i2]; simp?; linarith?)
+    apply (subst x64_bin_update_nth_error_other [of 6 l xpc u8_list l1 "xpc1+4" i3]; simp?; linarith?)
+    apply (subst x64_bin_update_nth_error_other [of 6 l xpc u8_list l1 "xpc1+5" i4]; simp?; linarith?)
+    done
+  apply ((erule case_option_eq_NE; simp?) | (erule ifE; erule conjE; simp))+
+  subgoal for reg dis src dst
+    apply (subst x64_bin_update_nth_error_other [of 6 l xpc u8_list l1 "xpc1+1" reg]; simp?; linarith?)
+    apply (subst x64_bin_update_nth_error_other [of 6 l xpc u8_list l1 "xpc1+2" dis]; simp?; linarith?)
+    done
+  apply ((erule case_option_eq_NE; simp?) | (erule ifE; erule conjE; simp))+
+  subgoal for reg dis src dst
+    apply (subst x64_bin_update_nth_error_other [of 6 l xpc u8_list l1 "xpc1+1" reg]; simp?; linarith?)
+    apply (subst x64_bin_update_nth_error_other [of 6 l xpc u8_list l1 "xpc1+2" dis]; simp?; linarith?)
+    done
+  apply ((erule case_option_eq_NE; simp?) | (erule ifE; erule conjE; simp))+
+  subgoal for reg d1 d2 d3 d4 dis src dst
+    apply (subst x64_bin_update_nth_error_other [of 6 l xpc u8_list l1 "xpc1+1" reg]; simp?; linarith?)
+    apply (subst x64_bin_update_nth_error_other [of 6 l xpc u8_list l1 "xpc1+2" d1]; simp?; linarith?)
+    apply (subst x64_bin_update_nth_error_other [of 6 l xpc u8_list l1 "xpc1+3" d2]; simp?; linarith?)
+    apply (subst x64_bin_update_nth_error_other [of 6 l xpc u8_list l1 "xpc1+4" d3]; simp?; linarith?)
+    apply (subst x64_bin_update_nth_error_other [of 6 l xpc u8_list l1 "xpc1+5" d4]; simp?; linarith?)
     done
   done
 
 lemma x64_encode_x64_decode_other:
   "(xpc1 + sz1 \<le> xpc \<or> xpc+sz \<le> xpc1) \<Longrightarrow>
-  x64_decode xpc l = Some (sz, Pjcc cond d0) \<Longrightarrow>
   x64_decode xpc1 l = Some (sz1, ins1) \<Longrightarrow>
-  sz = length u8_list \<Longrightarrow>
-  l1 = x64_bin_update (length u8_list) l xpc u8_list \<Longrightarrow>
+  length u8_list = 6 \<Longrightarrow>
+  sz = 6 \<Longrightarrow>
+  x64_bin_update 6 l xpc u8_list = l1 \<Longrightarrow>
     x64_decode xpc1 l1 = Some (sz1, ins1)"
   apply (simp add: x64_decode_def)
-  apply (erule case_option_eq_NE; simp?)
-  subgoal
-    using x64_decode_op_0x66_jcc_false by blast
-  subgoal a
-    apply (erule case_option_eq_NE; simp?)
-    subgoal for a1
-      using x64_bin_update_nth_error_other 
-      apply simp
-      done
-    subgoal for a1 apply (erule conjE)
-      using x64_bin_update_nth_error_other 
-      apply simp
-      by auto
-    subgoal for a1 apply (erule conjE)
-      using x64_bin_update_nth_error_other 
-      apply simp
-      by auto
-    subgoal for a1
-      apply (subgoal_tac "0 < sz1")
-      subgoal
-        using x64_bin_update_nth_error_other [of xpc1 sz1 xpc sz u8_list l 102]
-        apply simp
-        using x64_decode_op_0x66_jcc_other by blast
-      subgoal
-        apply (simp add: x64_decode_op_0x66_def nth_error_def;
-      (erule case_option_eq_NE; simp?)+)
-        done
-      done
-
-    subgoal for a1
-      apply (subgoal_tac "0 < sz1")
-      subgoal
-        using x64_bin_update_nth_error_other [of xpc1 sz1 xpc sz u8_list l 15]
-        apply simp
-        using x64_decode_op_0x0f_jcc_other by blast
-      subgoal
-        apply (simp add: x64_decode_op_0x0f_def nth_error_def;
-      (erule case_option_eq_NE; simp?)+)
-        done
-      done
-
-    subgoal for a1
-      apply (subgoal_tac "0 < sz1")
-      subgoal
-        using x64_bin_update_nth_error_other [of xpc1 sz1 xpc sz u8_list l a1]
-        apply simp
-        using x64_decode_op_not_rex_jcc_other by blast
-      subgoal
-        apply (simp add: x64_decode_op_not_rex_def nth_error_def;
-      (erule case_option_eq_NE; simp?)+)
-        done
-      done
-    subgoal for a1
-      sorry
-    subgoal for a1
-      sorry
+  apply (erule case_option_eq_NE; (simp add: split: if_split_asm)?)+
+  subgoal for h apply (erule conjE)
+    apply (subst x64_bin_update_nth_error_other [of 6 l xpc u8_list l1 xpc1 h]; simp?; linarith?)
     done
-  subgoal for a
-(**x64_decode_op_not_rex a xpc l = Some (length u8_list, Pjcc cond d0) \<Longrightarrow> False *)
-    sorry
-  subgoal for a
-    apply (cases "nth_error l xpc1"; simp add: split: if_split_asm)
+  subgoal for h apply (erule conjE)
+    apply (subst x64_bin_update_nth_error_other [of 6 l xpc u8_list l1 xpc1 h]; simp?; linarith?)
+    done
+  subgoal for h apply (erule conjE)
+    apply (subst x64_bin_update_nth_error_other [of 6 l xpc u8_list l1 xpc1 h]; simp?; linarith?)
+    done
+  subgoal for h
+    apply (subst x64_bin_update_nth_error_other [of 6 l xpc u8_list l1 xpc1 h]; simp?; linarith?)
+    subgoal using x64_encode_x64_decode_other_x64_decode_op_0x66_0 by blast
+    subgoal using x64_encode_x64_decode_other_x64_decode_op_0x66_1 by blast
+    done
+  subgoal for h
+    apply (subst x64_bin_update_nth_error_other [of 6 l xpc u8_list l1 xpc1 h]; simp?; linarith?)
+    subgoal using x64_encode_x64_decode_other_x64_decode_op_0x0f_0 by blast
+    subgoal using x64_encode_x64_decode_other_x64_decode_op_0x0f_1 by blast
+    done
+  subgoal for h
+    apply (subst x64_bin_update_nth_error_other [of 6 l xpc u8_list l1 xpc1 h]; simp?; linarith?)
+    subgoal using x64_encode_x64_decode_other_x64_decode_op_not_rex_0 by blast
+    subgoal using x64_encode_x64_decode_other_x64_decode_op_not_rex_1 by blast
+    done
+  subgoal for h
+    apply (erule case_option_eq_NE; simp?)+
+    subgoal for op
+      apply (erule ifE; erule conjE; simp)
+      subgoal
+        apply (subst x64_bin_update_nth_error_other [of 6 l xpc u8_list l1 xpc1 h]; simp?; linarith?)
+        apply (subst x64_bin_update_nth_error_other [of 6 l xpc u8_list l1 "xpc1+1" op]; simp?; linarith?)
+        done
+      apply (erule ifE; erule conjE; simp)
+      subgoal
+        by (erule case_option_eq_NE; simp?)+
+      apply (erule ifE; erule conjE; simp)
+      subgoal
+        by (erule case_option_eq_NE; simp?)
+
+      apply (erule ifE; erule conjE; simp)
+      subgoal
+        apply (erule case_option_eq_NE; simp?)+
+        subgoal for i1 i2 i3 i4 i5 i6 i7 i8 dst imm
+          apply (subst x64_bin_update_nth_error_other [of 6 l xpc u8_list l1 xpc1 h]; simp?; linarith?)
+          apply (subst x64_bin_update_nth_error_other [of 6 l xpc u8_list l1 "xpc1+1" op]; simp?; linarith?)
+          apply (subst x64_bin_update_nth_error_other [of 6 l xpc u8_list l1 "xpc1+2" i1]; simp?; linarith?)
+          apply (subst x64_bin_update_nth_error_other [of 6 l xpc u8_list l1 "xpc1+3" i2]; simp?; linarith?)
+          apply (subst x64_bin_update_nth_error_other [of 6 l xpc u8_list l1 "xpc1+4" i3]; simp?; linarith?)
+          apply (subst x64_bin_update_nth_error_other [of 6 l xpc u8_list l1 "xpc1+5" i4]; simp?; linarith?)
+          apply (subst x64_bin_update_nth_error_other [of 6 l xpc u8_list l1 "xpc1+6" i5]; simp?; linarith?)
+          apply (subst x64_bin_update_nth_error_other [of 6 l xpc u8_list l1 "xpc1+7" i6]; simp?; linarith?)
+          apply (subst x64_bin_update_nth_error_other [of 6 l xpc u8_list l1 "xpc1+8" i7]; simp?; linarith?)
+          apply (subst x64_bin_update_nth_error_other [of 6 l xpc u8_list l1 "xpc1+9" i8]; simp?; linarith?)
+          done
+        done
+
+      apply (erule ifE; erule conjE; simp)
+      subgoal
+        apply (erule case_option_eq_NE; simp?)+
+        subgoal for i1 i2 i3 i4 imm
+          apply (subst x64_bin_update_nth_error_other [of 6 l xpc u8_list l1 xpc1 h]; simp?; linarith?)
+          apply (subst x64_bin_update_nth_error_other [of 6 l xpc u8_list l1 "xpc1+1" op]; simp?; linarith?)
+          apply (subst x64_bin_update_nth_error_other [of 6 l xpc u8_list l1 "xpc1+2" i1]; simp?; linarith?)
+          apply (subst x64_bin_update_nth_error_other [of 6 l xpc u8_list l1 "xpc1+3" i2]; simp?; linarith?)
+          apply (subst x64_bin_update_nth_error_other [of 6 l xpc u8_list l1 "xpc1+4" i3]; simp?; linarith?)
+          apply (subst x64_bin_update_nth_error_other [of 6 l xpc u8_list l1 "xpc1+5" i4]; simp?; linarith?)
+          done
+        done
+
+      apply (erule ifE; erule conjE; simp)
+      subgoal
+        apply ((erule case_option_eq_NE; simp?) | (erule ifE; erule conjE; simp))+
+        subgoal for op1 dst
+          apply (subst x64_bin_update_nth_error_other [of 6 l xpc u8_list l1 xpc1 h]; simp?; linarith?)
+          apply (subst x64_bin_update_nth_error_other [of 6 l xpc u8_list l1 "xpc1+1" op]; simp?; linarith?)
+          apply (subst x64_bin_update_nth_error_other [of 6 l xpc u8_list l1 "xpc1+2" op1]; simp?; linarith?)
+          done
+        subgoal for op1
+          apply ((erule case_option_eq_NE; simp?) | (erule ifE; erule conjE; simp))+
+          subgoal for reg t src dst
+            apply (subst x64_bin_update_nth_error_other [of 6 l xpc u8_list l1 xpc1 h]; simp?; linarith?)
+            apply (subst x64_bin_update_nth_error_other [of 6 l xpc u8_list l1 "xpc1+1" op]; simp?; linarith?)
+            apply (subst x64_bin_update_nth_error_other [of 6 l xpc u8_list l1 "xpc1+2" op1]; simp?; linarith?)
+            apply (subst x64_bin_update_nth_error_other [of 6 l xpc u8_list l1 "xpc1+3" reg]; simp?; linarith?)
+            done
+          done
+        done
+
+      apply ((erule case_option_eq_NE; simp?) | (erule ifE; erule conjE; simp))+
+      subgoal for reg src dst
+          apply (subst x64_bin_update_nth_error_other [of 6 l xpc u8_list l1 xpc1 h]; simp?; linarith?)
+          apply (subst x64_bin_update_nth_error_other [of 6 l xpc u8_list l1 "xpc1+1" op]; simp?; linarith?)
+          apply (subst x64_bin_update_nth_error_other [of 6 l xpc u8_list l1 "xpc1+2" reg]; simp?; linarith?)
+          done
+        subgoal for reg
+          apply ((erule case_option_eq_NE; simp?) | (erule ifE; erule conjE; simp))+
+          subgoal for dis src dst
+            apply (subst x64_bin_update_nth_error_other [of 6 l xpc u8_list l1 xpc1 h]; simp?; linarith?)
+            apply (subst x64_bin_update_nth_error_other [of 6 l xpc u8_list l1 "xpc1+1" op]; simp?; linarith?)
+            apply (subst x64_bin_update_nth_error_other [of 6 l xpc u8_list l1 "xpc1+2" reg]; simp?; linarith?)
+            apply (subst x64_bin_update_nth_error_other [of 6 l xpc u8_list l1 "xpc1+3" dis]; simp?; linarith?)
+            done
+
+          apply ((erule case_option_eq_NE; simp?) | (erule ifE; erule conjE; simp))+
+          subgoal for d1 d2 d3 d4 dis src rb
+            apply (subst x64_bin_update_nth_error_other [of 6 l xpc u8_list l1 xpc1 h]; simp?; linarith?)
+            apply (subst x64_bin_update_nth_error_other [of 6 l xpc u8_list l1 "xpc1+1" op]; simp?; linarith?)
+            apply (subst x64_bin_update_nth_error_other [of 6 l xpc u8_list l1 "xpc1+2" reg]; simp?; linarith?)
+            apply (subst x64_bin_update_nth_error_other [of 6 l xpc u8_list l1 "xpc1+3" d1]; simp?; linarith?)
+            apply (subst x64_bin_update_nth_error_other [of 6 l xpc u8_list l1 "xpc1+4" d2]; simp?; linarith?)
+            apply (subst x64_bin_update_nth_error_other [of 6 l xpc u8_list l1 "xpc1+5" d3]; simp?; linarith?)
+            apply (subst x64_bin_update_nth_error_other [of 6 l xpc u8_list l1 "xpc1+6" d4]; simp?; linarith?)
+            done
+
+          apply ((erule case_option_eq_NE; simp?) | (erule ifE; erule conjE; simp))+
+          subgoal for sib d1 d2 d3 d4 dis src ri rb
+            apply (subst x64_bin_update_nth_error_other [of 6 l xpc u8_list l1 xpc1 h]; simp?; linarith?)
+            apply (subst x64_bin_update_nth_error_other [of 6 l xpc u8_list l1 "xpc1+1" op]; simp?; linarith?)
+            apply (subst x64_bin_update_nth_error_other [of 6 l xpc u8_list l1 "xpc1+2" reg]; simp?; linarith?)
+            apply (subst x64_bin_update_nth_error_other [of 6 l xpc u8_list l1 "xpc1+3" sib]; simp?; linarith?)
+            apply (subst x64_bin_update_nth_error_other [of 6 l xpc u8_list l1 "xpc1+4" d1]; simp?; linarith?)
+            apply (subst x64_bin_update_nth_error_other [of 6 l xpc u8_list l1 "xpc1+5" d2]; simp?; linarith?)
+            apply (subst x64_bin_update_nth_error_other [of 6 l xpc u8_list l1 "xpc1+6" d3]; simp?; linarith?)
+            apply (subst x64_bin_update_nth_error_other [of 6 l xpc u8_list l1 "xpc1+7" d4]; simp?; linarith?)
+            done
+          done
+        subgoal for reg
+          apply ((erule case_option_eq_NE; simp?) | (erule ifE; erule conjE; simp))+
+          subgoal for src dst
+            apply (subst x64_bin_update_nth_error_other [of 6 l xpc u8_list l1 xpc1 h]; simp?; linarith?)
+            apply (subst x64_bin_update_nth_error_other [of 6 l xpc u8_list l1 "xpc1+1" op]; simp?; linarith?)
+            apply (subst x64_bin_update_nth_error_other [of 6 l xpc u8_list l1 "xpc1+2" reg]; simp?; linarith?)
+            done
+
+          subgoal
+            apply ((erule case_option_eq_NE; simp?) | (erule ifE; erule conjE; simp))+
+            subgoal for sib d1 d2 d3 d4 dis src ri rb
+              apply (subst x64_bin_update_nth_error_other [of 6 l xpc u8_list l1 xpc1 h]; simp?; linarith?)
+              apply (subst x64_bin_update_nth_error_other [of 6 l xpc u8_list l1 "xpc1+1" op]; simp?; linarith?)
+              apply (subst x64_bin_update_nth_error_other [of 6 l xpc u8_list l1 "xpc1+2" reg]; simp?; linarith?)
+              apply (subst x64_bin_update_nth_error_other [of 6 l xpc u8_list l1 "xpc1+3" sib]; simp?; linarith?)
+              apply (subst x64_bin_update_nth_error_other [of 6 l xpc u8_list l1 "xpc1+4" d1]; simp?; linarith?)
+              apply (subst x64_bin_update_nth_error_other [of 6 l xpc u8_list l1 "xpc1+5" d2]; simp?; linarith?)
+              apply (subst x64_bin_update_nth_error_other [of 6 l xpc u8_list l1 "xpc1+6" d3]; simp?; linarith?)
+              apply (subst x64_bin_update_nth_error_other [of 6 l xpc u8_list l1 "xpc1+7" d4]; simp?; linarith?)
+              done
+            done
+
+          apply ((erule case_option_eq_NE; simp?) | (erule ifE; erule conjE; simp))+
+          subgoal for src dst
+            apply (subst x64_bin_update_nth_error_other [of 6 l xpc u8_list l1 xpc1 h]; simp?; linarith?)
+            apply (subst x64_bin_update_nth_error_other [of 6 l xpc u8_list l1 "xpc1+1" op]; simp?; linarith?)
+            apply (subst x64_bin_update_nth_error_other [of 6 l xpc u8_list l1 "xpc1+2" reg]; simp?; linarith?)
+            done
+
+          apply ((erule case_option_eq_NE; simp?) | (erule ifE; erule conjE; simp))+
+          subgoal for src dst
+            apply (subst x64_bin_update_nth_error_other [of 6 l xpc u8_list l1 xpc1 h]; simp?; linarith?)
+            apply (subst x64_bin_update_nth_error_other [of 6 l xpc u8_list l1 "xpc1+1" op]; simp?; linarith?)
+            apply (subst x64_bin_update_nth_error_other [of 6 l xpc u8_list l1 "xpc1+2" reg]; simp?; linarith?)
+            done
+
+          apply ((erule case_option_eq_NE; simp?) | (erule ifE; erule conjE; simp))+
+          subgoal for src dst
+            apply (subst x64_bin_update_nth_error_other [of 6 l xpc u8_list l1 xpc1 h]; simp?; linarith?)
+            apply (subst x64_bin_update_nth_error_other [of 6 l xpc u8_list l1 "xpc1+1" op]; simp?; linarith?)
+            apply (subst x64_bin_update_nth_error_other [of 6 l xpc u8_list l1 "xpc1+2" reg]; simp?; linarith?)
+            done
+
+          apply ((erule case_option_eq_NE; simp?) | (erule ifE; erule conjE; simp))+
+          subgoal for dst
+            apply (subst x64_bin_update_nth_error_other [of 6 l xpc u8_list l1 xpc1 h]; simp?; linarith?)
+            apply (subst x64_bin_update_nth_error_other [of 6 l xpc u8_list l1 "xpc1+1" op]; simp?; linarith?)
+            apply (subst x64_bin_update_nth_error_other [of 6 l xpc u8_list l1 "xpc1+2" reg]; simp?; linarith?)
+            done
+          subgoal
+            apply ((erule case_option_eq_NE; simp?) | (erule ifE; erule conjE; simp))+
+            subgoal for dst
+              apply (subst x64_bin_update_nth_error_other [of 6 l xpc u8_list l1 xpc1 h]; simp?; linarith?)
+              apply (subst x64_bin_update_nth_error_other [of 6 l xpc u8_list l1 "xpc1+1" op]; simp?; linarith?)
+              apply (subst x64_bin_update_nth_error_other [of 6 l xpc u8_list l1 "xpc1+2" reg]; simp?; linarith?)
+              done
+            apply ((erule case_option_eq_NE; simp?) | (erule ifE; erule conjE; simp))+
+            subgoal for dst
+              apply (subst x64_bin_update_nth_error_other [of 6 l xpc u8_list l1 xpc1 h]; simp?; linarith?)
+              apply (subst x64_bin_update_nth_error_other [of 6 l xpc u8_list l1 "xpc1+1" op]; simp?; linarith?)
+              apply (subst x64_bin_update_nth_error_other [of 6 l xpc u8_list l1 "xpc1+2" reg]; simp?; linarith?)
+              done
+
+
+            apply ((erule case_option_eq_NE; simp?) | (erule ifE; erule conjE; simp))+
+            subgoal for dst
+              apply (subst x64_bin_update_nth_error_other [of 6 l xpc u8_list l1 xpc1 h]; simp?; linarith?)
+              apply (subst x64_bin_update_nth_error_other [of 6 l xpc u8_list l1 "xpc1+1" op]; simp?; linarith?)
+              apply (subst x64_bin_update_nth_error_other [of 6 l xpc u8_list l1 "xpc1+2" reg]; simp?; linarith?)
+              done
+
+            apply ((erule case_option_eq_NE; simp?) | (erule ifE; erule conjE; simp))+
+            subgoal for dst
+              apply (subst x64_bin_update_nth_error_other [of 6 l xpc u8_list l1 xpc1 h]; simp?; linarith?)
+              apply (subst x64_bin_update_nth_error_other [of 6 l xpc u8_list l1 "xpc1+1" op]; simp?; linarith?)
+              apply (subst x64_bin_update_nth_error_other [of 6 l xpc u8_list l1 "xpc1+2" reg]; simp?; linarith?)
+              done
+
+            apply ((erule case_option_eq_NE; simp?) | (erule ifE; erule conjE; simp))+
+            subgoal for i1 i2 i3 i4 dst imm
+              apply (subst x64_bin_update_nth_error_other [of 6 l xpc u8_list l1 xpc1 h]; simp?; linarith?)
+              apply (subst x64_bin_update_nth_error_other [of 6 l xpc u8_list l1 "xpc1+1" op]; simp?; linarith?)
+              apply (subst x64_bin_update_nth_error_other [of 6 l xpc u8_list l1 "xpc1+2" reg]; simp?; linarith?)
+              apply (subst x64_bin_update_nth_error_other [of 6 l xpc u8_list l1 "xpc1+3" i1]; simp?; linarith?)
+              apply (subst x64_bin_update_nth_error_other [of 6 l xpc u8_list l1 "xpc1+4" i2]; simp?; linarith?)
+              apply (subst x64_bin_update_nth_error_other [of 6 l xpc u8_list l1 "xpc1+5" i3]; simp?; linarith?)
+              apply (subst x64_bin_update_nth_error_other [of 6 l xpc u8_list l1 "xpc1+6" i4]; simp?; linarith?)
+              done
+            done
+
+          apply ((erule case_option_eq_NE; simp?) | (erule ifE; erule conjE; simp))+
+          subgoal for src dst
+            apply (subst x64_bin_update_nth_error_other [of 6 l xpc u8_list l1 xpc1 h]; simp?; linarith?)
+            apply (subst x64_bin_update_nth_error_other [of 6 l xpc u8_list l1 "xpc1+1" op]; simp?; linarith?)
+            apply (subst x64_bin_update_nth_error_other [of 6 l xpc u8_list l1 "xpc1+2" reg]; simp?; linarith?)
+            done
+
+          apply ((erule case_option_eq_NE; simp?) | (erule ifE; erule conjE; simp))+
+          subgoal for src dst
+            apply (subst x64_bin_update_nth_error_other [of 6 l xpc u8_list l1 xpc1 h]; simp?; linarith?)
+            apply (subst x64_bin_update_nth_error_other [of 6 l xpc u8_list l1 "xpc1+1" op]; simp?; linarith?)
+            apply (subst x64_bin_update_nth_error_other [of 6 l xpc u8_list l1 "xpc1+2" reg]; simp?; linarith?)
+            done
+
+          apply ((erule case_option_eq_NE; simp?) | (erule ifE; erule conjE; simp))+
+          subgoal for src dst
+            apply (subst x64_bin_update_nth_error_other [of 6 l xpc u8_list l1 xpc1 h]; simp?; linarith?)
+            apply (subst x64_bin_update_nth_error_other [of 6 l xpc u8_list l1 "xpc1+1" op]; simp?; linarith?)
+            apply (subst x64_bin_update_nth_error_other [of 6 l xpc u8_list l1 "xpc1+2" reg]; simp?; linarith?)
+            done
+
+          apply ((erule case_option_eq_NE; simp?) | (erule ifE; erule conjE; simp))+
+          subgoal for dst
+            apply (subst x64_bin_update_nth_error_other [of 6 l xpc u8_list l1 xpc1 h]; simp?; linarith?)
+            apply (subst x64_bin_update_nth_error_other [of 6 l xpc u8_list l1 "xpc1+1" op]; simp?; linarith?)
+            apply (subst x64_bin_update_nth_error_other [of 6 l xpc u8_list l1 "xpc1+2" reg]; simp?; linarith?)
+            done
+          subgoal
+            apply ((erule case_option_eq_NE; simp?) | (erule ifE; erule conjE; simp))+
+            subgoal for dst
+              apply (subst x64_bin_update_nth_error_other [of 6 l xpc u8_list l1 xpc1 h]; simp?; linarith?)
+              apply (subst x64_bin_update_nth_error_other [of 6 l xpc u8_list l1 "xpc1+1" op]; simp?; linarith?)
+              apply (subst x64_bin_update_nth_error_other [of 6 l xpc u8_list l1 "xpc1+2" reg]; simp?; linarith?)
+              done
+
+            apply ((erule case_option_eq_NE; simp?) | (erule ifE; erule conjE; simp))+
+            subgoal for dst
+              apply (subst x64_bin_update_nth_error_other [of 6 l xpc u8_list l1 xpc1 h]; simp?; linarith?)
+              apply (subst x64_bin_update_nth_error_other [of 6 l xpc u8_list l1 "xpc1+1" op]; simp?; linarith?)
+              apply (subst x64_bin_update_nth_error_other [of 6 l xpc u8_list l1 "xpc1+2" reg]; simp?; linarith?)
+              done
+            done
+          apply ((erule case_option_eq_NE; simp?) | (erule ifE; erule conjE; simp))+
+          subgoal for dst
+            apply (subst x64_bin_update_nth_error_other [of 6 l xpc u8_list l1 xpc1 h]; simp?; linarith?)
+            apply (subst x64_bin_update_nth_error_other [of 6 l xpc u8_list l1 "xpc1+1" op]; simp?; linarith?)
+            apply (subst x64_bin_update_nth_error_other [of 6 l xpc u8_list l1 "xpc1+2" reg]; simp?; linarith?)
+            done
+
+          apply ((erule case_option_eq_NE; simp?) | (erule ifE; erule conjE; simp))+
+          subgoal for dst
+            apply (subst x64_bin_update_nth_error_other [of 6 l xpc u8_list l1 xpc1 h]; simp?; linarith?)
+            apply (subst x64_bin_update_nth_error_other [of 6 l xpc u8_list l1 "xpc1+1" op]; simp?; linarith?)
+            apply (subst x64_bin_update_nth_error_other [of 6 l xpc u8_list l1 "xpc1+2" reg]; simp?; linarith?)
+            done
+
+          apply ((erule case_option_eq_NE; simp?) | (erule ifE; erule conjE; simp))+
+          subgoal for sib d1 d2 d3 d4 dis
+            apply (erule conjE)
+            apply ((erule case_option_eq_NE; simp?) | (erule ifE; erule conjE; simp))+
+            subgoal for ri rb
+              apply (subst x64_bin_update_nth_error_other [of 6 l xpc u8_list l1 xpc1 h]; simp?; linarith?)
+              apply (subst x64_bin_update_nth_error_other [of 6 l xpc u8_list l1 "xpc1+1" op]; simp?; linarith?)
+              apply (subst x64_bin_update_nth_error_other [of 6 l xpc u8_list l1 "xpc1+2" reg]; simp?; linarith?)
+              apply (subst x64_bin_update_nth_error_other [of 6 l xpc u8_list l1 "xpc1+3" sib]; simp?; linarith?)
+              apply (subst x64_bin_update_nth_error_other [of 6 l xpc u8_list l1 "xpc1+4" d1]; simp?; linarith?)
+              apply (subst x64_bin_update_nth_error_other [of 6 l xpc u8_list l1 "xpc1+5" d2]; simp?; linarith?)
+              apply (subst x64_bin_update_nth_error_other [of 6 l xpc u8_list l1 "xpc1+6" d3]; simp?; linarith?)
+              apply (subst x64_bin_update_nth_error_other [of 6 l xpc u8_list l1 "xpc1+7" d4]; simp?; linarith?)
+              done
+            done
+
+          apply ((erule case_option_eq_NE; simp?) | (erule ifE; erule conjE; simp))+
+          subgoal for i1 i2 i3 i4 dst imm dis
+            apply (subst x64_bin_update_nth_error_other [of 6 l xpc u8_list l1 xpc1 h]; simp?; linarith?)
+            apply (subst x64_bin_update_nth_error_other [of 6 l xpc u8_list l1 "xpc1+1" op]; simp?; linarith?)
+            apply (subst x64_bin_update_nth_error_other [of 6 l xpc u8_list l1 "xpc1+2" reg]; simp?; linarith?)
+            apply (subst x64_bin_update_nth_error_other [of 6 l xpc u8_list l1 "xpc1+3" dis]; simp?; linarith?)
+            apply (subst x64_bin_update_nth_error_other [of 6 l xpc u8_list l1 "4+xpc1" i1]; simp?; linarith?)
+            apply (subst x64_bin_update_nth_error_other [of 6 l xpc u8_list l1 "5+xpc1" i2]; simp?; linarith?)
+            apply (subst x64_bin_update_nth_error_other [of 6 l xpc u8_list l1 "6+xpc1" i3]; simp?; linarith?)
+            apply (subst x64_bin_update_nth_error_other [of 6 l xpc u8_list l1 "7+xpc1" i4]; simp?; linarith?)
+            done
+          subgoal for i1 i2 i3 i4 dst imm
+            apply ((erule case_option_eq_NE; simp?) | (erule ifE; erule conjE; simp))+
+            subgoal for d1 d2 d3 d4 dis
+              apply (subst x64_bin_update_nth_error_other [of 6 l xpc u8_list l1 xpc1 h]; simp?; linarith?)
+              apply (subst x64_bin_update_nth_error_other [of 6 l xpc u8_list l1 "xpc1+1" op]; simp?; linarith?)
+              apply (subst x64_bin_update_nth_error_other [of 6 l xpc u8_list l1 "xpc1+2" reg]; simp?; linarith?)
+              apply (subst x64_bin_update_nth_error_other [of 6 l xpc u8_list l1 "7+xpc1" i1]; simp?; linarith?)
+              apply (subst x64_bin_update_nth_error_other [of 6 l xpc u8_list l1 "8+xpc1" i2]; simp?; linarith?)
+              apply (subst x64_bin_update_nth_error_other [of 6 l xpc u8_list l1 "9+xpc1" i3]; simp?; linarith?)
+              apply (subst x64_bin_update_nth_error_other [of 6 l xpc u8_list l1 "10+xpc1" i4]; simp?; linarith?)
+              apply (subst x64_bin_update_nth_error_other [of 6 l xpc u8_list l1 "xpc1+3" d1]; simp?; linarith?)
+              apply (subst x64_bin_update_nth_error_other [of 6 l xpc u8_list l1 "xpc1+4" d2]; simp?; linarith?)
+              apply (subst x64_bin_update_nth_error_other [of 6 l xpc u8_list l1 "xpc1+5" d3]; simp?; linarith?)
+              apply (subst x64_bin_update_nth_error_other [of 6 l xpc u8_list l1 "xpc1+6" d4]; simp?; linarith?)
+              done
+            done
+
+          apply ((erule case_option_eq_NE; simp?) | (erule ifE; erule conjE; simp))+
+          subgoal for dst i1 i2 i3 i4 imm
+            apply (subst x64_bin_update_nth_error_other [of 6 l xpc u8_list l1 xpc1 h]; simp?; linarith?)
+            apply (subst x64_bin_update_nth_error_other [of 6 l xpc u8_list l1 "xpc1+1" op]; simp?; linarith?)
+            apply (subst x64_bin_update_nth_error_other [of 6 l xpc u8_list l1 "xpc1+2" reg]; simp?; linarith?)
+            apply (subst x64_bin_update_nth_error_other [of 6 l xpc u8_list l1 "xpc1+3" i1]; simp?; linarith?)
+            apply (subst x64_bin_update_nth_error_other [of 6 l xpc u8_list l1 "xpc1+4" i2]; simp?; linarith?)
+            apply (subst x64_bin_update_nth_error_other [of 6 l xpc u8_list l1 "xpc1+5" i3]; simp?; linarith?)
+            apply (subst x64_bin_update_nth_error_other [of 6 l xpc u8_list l1 "xpc1+6" i4]; simp?; linarith?)
+            done
+
+           apply ((erule case_option_eq_NE; simp?) | (erule ifE; erule conjE; simp))+
+          subgoal for sib d1 d2 d3 d4 dis
+            apply (erule conjE)
+            apply ((erule case_option_eq_NE; simp?) | (erule ifE; erule conjE; simp))+
+            subgoal for i1 i2 i3 i4 imm ri rb
+              apply (subst x64_bin_update_nth_error_other [of 6 l xpc u8_list l1 xpc1 h]; simp?; linarith?)
+              apply (subst x64_bin_update_nth_error_other [of 6 l xpc u8_list l1 "xpc1+1" op]; simp?; linarith?)
+              apply (subst x64_bin_update_nth_error_other [of 6 l xpc u8_list l1 "xpc1+2" reg]; simp?; linarith?)
+              apply (subst x64_bin_update_nth_error_other [of 6 l xpc u8_list l1 "xpc1+3" sib]; simp?; linarith?)
+              apply (subst x64_bin_update_nth_error_other [of 6 l xpc u8_list l1 "xpc1+4" d1]; simp?; linarith?)
+              apply (subst x64_bin_update_nth_error_other [of 6 l xpc u8_list l1 "xpc1+5" d2]; simp?; linarith?)
+              apply (subst x64_bin_update_nth_error_other [of 6 l xpc u8_list l1 "xpc1+6" d3]; simp?; linarith?)
+              apply (subst x64_bin_update_nth_error_other [of 6 l xpc u8_list l1 "xpc1+7" d4]; simp?; linarith?)
+              apply (subst x64_bin_update_nth_error_other [of 6 l xpc u8_list l1 "xpc1+8" i1]; simp?; linarith?)
+              apply (subst x64_bin_update_nth_error_other [of 6 l xpc u8_list l1 "xpc1+9" i2]; simp?; linarith?)
+              apply (subst x64_bin_update_nth_error_other [of 6 l xpc u8_list l1 "xpc1+10" i3]; simp?; linarith?)
+              apply (subst x64_bin_update_nth_error_other [of 6 l xpc u8_list l1 "xpc1+11" i4]; simp?; linarith?)
+              done
+            done
+
+          apply ((erule case_option_eq_NE; simp?) | (erule ifE; erule conjE; simp))+
+          subgoal for imm dst
+            apply (subst x64_bin_update_nth_error_other [of 6 l xpc u8_list l1 xpc1 h]; simp?; linarith?)
+            apply (subst x64_bin_update_nth_error_other [of 6 l xpc u8_list l1 "xpc1+1" op]; simp?; linarith?)
+            apply (subst x64_bin_update_nth_error_other [of 6 l xpc u8_list l1 "xpc1+2" reg]; simp?; linarith?)
+            apply (subst x64_bin_update_nth_error_other [of 6 l xpc u8_list l1 "xpc1+3" imm]; simp?; linarith?)
+            done
+
+          subgoal for imm
+            apply ((erule case_option_eq_NE; simp?) | (erule ifE; erule conjE; simp))+
+            subgoal for dst
+              apply (subst x64_bin_update_nth_error_other [of 6 l xpc u8_list l1 xpc1 h]; simp?; linarith?)
+              apply (subst x64_bin_update_nth_error_other [of 6 l xpc u8_list l1 "xpc1+1" op]; simp?; linarith?)
+              apply (subst x64_bin_update_nth_error_other [of 6 l xpc u8_list l1 "xpc1+2" reg]; simp?; linarith?)
+              apply (subst x64_bin_update_nth_error_other [of 6 l xpc u8_list l1 "xpc1+3" imm]; simp?; linarith?)
+              done
+            apply ((erule case_option_eq_NE; simp?) | (erule ifE; erule conjE; simp))+
+            subgoal for dst
+              apply (subst x64_bin_update_nth_error_other [of 6 l xpc u8_list l1 xpc1 h]; simp?; linarith?)
+              apply (subst x64_bin_update_nth_error_other [of 6 l xpc u8_list l1 "xpc1+1" op]; simp?; linarith?)
+              apply (subst x64_bin_update_nth_error_other [of 6 l xpc u8_list l1 "xpc1+2" reg]; simp?; linarith?)
+              apply (subst x64_bin_update_nth_error_other [of 6 l xpc u8_list l1 "xpc1+3" imm]; simp?; linarith?)
+              done
+            done
+
+          apply ((erule case_option_eq_NE; simp?) | (erule ifE; erule conjE; simp))+
+          subgoal for dis src dst
+            apply (subst x64_bin_update_nth_error_other [of 6 l xpc u8_list l1 xpc1 h]; simp?; linarith?)
+            apply (subst x64_bin_update_nth_error_other [of 6 l xpc u8_list l1 "xpc1+1" op]; simp?; linarith?)
+            apply (subst x64_bin_update_nth_error_other [of 6 l xpc u8_list l1 "xpc1+2" reg]; simp?; linarith?)
+            apply (subst x64_bin_update_nth_error_other [of 6 l xpc u8_list l1 "xpc1+3" dis]; simp?; linarith?)
+            done
+          subgoal 
+            apply ((erule case_option_eq_NE; simp?) | (erule ifE; erule conjE; simp))+
+            subgoal for d1 d2 d3 d4 dis src dst
+              apply (subst x64_bin_update_nth_error_other [of 6 l xpc u8_list l1 xpc1 h]; simp?; linarith?)
+              apply (subst x64_bin_update_nth_error_other [of 6 l xpc u8_list l1 "xpc1+1" op]; simp?; linarith?)
+              apply (subst x64_bin_update_nth_error_other [of 6 l xpc u8_list l1 "xpc1+2" reg]; simp?; linarith?)
+              apply (subst x64_bin_update_nth_error_other [of 6 l xpc u8_list l1 "xpc1+3" d1]; simp?; linarith?)
+              apply (subst x64_bin_update_nth_error_other [of 6 l xpc u8_list l1 "xpc1+4" d2]; simp?; linarith?)
+              apply (subst x64_bin_update_nth_error_other [of 6 l xpc u8_list l1 "xpc1+5" d3]; simp?; linarith?)
+              apply (subst x64_bin_update_nth_error_other [of 6 l xpc u8_list l1 "xpc1+6" d4]; simp?; linarith?)
+              done
+
+            apply ((erule case_option_eq_NE; simp?) | (erule ifE; erule conjE; simp))+
+            subgoal for sib d1 d2 d3 d4 dis src ri rb
+              apply (subst x64_bin_update_nth_error_other [of 6 l xpc u8_list l1 xpc1 h]; simp?; linarith?)
+              apply (subst x64_bin_update_nth_error_other [of 6 l xpc u8_list l1 "xpc1+1" op]; simp?; linarith?)
+              apply (subst x64_bin_update_nth_error_other [of 6 l xpc u8_list l1 "xpc1+2" reg]; simp?; linarith?)
+              apply (subst x64_bin_update_nth_error_other [of 6 l xpc u8_list l1 "xpc1+3" sib]; simp?; linarith?)
+              apply (subst x64_bin_update_nth_error_other [of 6 l xpc u8_list l1 "xpc1+4" d1]; simp?; linarith?)
+              apply (subst x64_bin_update_nth_error_other [of 6 l xpc u8_list l1 "xpc1+5" d2]; simp?; linarith?)
+              apply (subst x64_bin_update_nth_error_other [of 6 l xpc u8_list l1 "xpc1+6" d3]; simp?; linarith?)
+              apply (subst x64_bin_update_nth_error_other [of 6 l xpc u8_list l1 "xpc1+7" d4]; simp?; linarith?)
+              done
+            done
+
+          apply ((erule case_option_eq_NE; simp?) | (erule ifE; erule conjE; simp))+
+          subgoal for dis src dst
+            apply (subst x64_bin_update_nth_error_other [of 6 l xpc u8_list l1 xpc1 h]; simp?; linarith?)
+            apply (subst x64_bin_update_nth_error_other [of 6 l xpc u8_list l1 "xpc1+1" op]; simp?; linarith?)
+            apply (subst x64_bin_update_nth_error_other [of 6 l xpc u8_list l1 "xpc1+2" reg]; simp?; linarith?)
+            apply (subst x64_bin_update_nth_error_other [of 6 l xpc u8_list l1 "xpc1+3" dis]; simp?; linarith?)
+            done
+          subgoal
+            apply ((erule case_option_eq_NE; simp?) | (erule ifE; erule conjE; simp))+
+            subgoal for d1 d2 d3 d4 dis src dst
+              apply (subst x64_bin_update_nth_error_other [of 6 l xpc u8_list l1 xpc1 h]; simp?; linarith?)
+              apply (subst x64_bin_update_nth_error_other [of 6 l xpc u8_list l1 "xpc1+1" op]; simp?; linarith?)
+              apply (subst x64_bin_update_nth_error_other [of 6 l xpc u8_list l1 "xpc1+2" reg]; simp?; linarith?)
+              apply (subst x64_bin_update_nth_error_other [of 6 l xpc u8_list l1 "xpc1+3" d1]; simp?; linarith?)
+              apply (subst x64_bin_update_nth_error_other [of 6 l xpc u8_list l1 "xpc1+4" d2]; simp?; linarith?)
+              apply (subst x64_bin_update_nth_error_other [of 6 l xpc u8_list l1 "xpc1+5" d3]; simp?; linarith?)
+              apply (subst x64_bin_update_nth_error_other [of 6 l xpc u8_list l1 "xpc1+6" d4]; simp?; linarith?)
+              done
+            done
+          done
+        done
+      done
+
+
+  subgoal for h
+    apply ((erule case_option_eq_NE; simp?) | (erule ifE; erule conjE; simp))+
+    subgoal for op i1 i2 i3 i4 i5 i6 i7 i8 dst imm
+      apply (subst x64_bin_update_nth_error_other [of 6 l xpc u8_list l1 xpc1 h]; simp?; linarith?)
+      apply (subst x64_bin_update_nth_error_other [of 6 l xpc u8_list l1 "xpc1+1" op]; simp?; linarith?)
+      apply (subst x64_bin_update_nth_error_other [of 6 l xpc u8_list l1 "xpc1+2" i1]; simp?; linarith?)
+      apply (subst x64_bin_update_nth_error_other [of 6 l xpc u8_list l1 "xpc1+3" i2]; simp?; linarith?)
+      apply (subst x64_bin_update_nth_error_other [of 6 l xpc u8_list l1 "xpc1+4" i3]; simp?; linarith?)
+      apply (subst x64_bin_update_nth_error_other [of 6 l xpc u8_list l1 "xpc1+5" i4]; simp?; linarith?)
+      apply (subst x64_bin_update_nth_error_other [of 6 l xpc u8_list l1 "xpc1+6" i5]; simp?; linarith?)
+      apply (subst x64_bin_update_nth_error_other [of 6 l xpc u8_list l1 "xpc1+7" i6]; simp?; linarith?)
+      apply (subst x64_bin_update_nth_error_other [of 6 l xpc u8_list l1 "xpc1+8" i7]; simp?; linarith?)
+      apply (subst x64_bin_update_nth_error_other [of 6 l xpc u8_list l1 "xpc1+9" i8]; simp?; linarith?)
+      done
+    subgoal for op
+      apply ((erule case_option_eq_NE; simp?) | (erule ifE; erule conjE; simp))+
+      subgoal for op1 dst
+        apply (subst x64_bin_update_nth_error_other [of 6 l xpc u8_list l1 xpc1 h]; simp?; linarith?)
+        apply (subst x64_bin_update_nth_error_other [of 6 l xpc u8_list l1 "xpc1+1" op]; simp?; linarith?)
+        apply (subst x64_bin_update_nth_error_other [of 6 l xpc u8_list l1 "xpc1+2" op1]; simp?; linarith?)
+        done
+      subgoal for op1
+        apply ((erule case_option_eq_NE; simp?) | (erule ifE; erule conjE; simp))+
+        subgoal for reg t src dst
+          apply (subst x64_bin_update_nth_error_other [of 6 l xpc u8_list l1 xpc1 h]; simp?; linarith?)
+          apply (rule conjI, rule impI)
+          subgoal by blast
+          apply (subst x64_bin_update_nth_error_other [of 6 l xpc u8_list l1 "xpc1+1" op]; simp?; linarith?)
+          apply (subst x64_bin_update_nth_error_other [of 6 l xpc u8_list l1 "xpc1+2" op1]; simp?; linarith?)
+          apply (subst x64_bin_update_nth_error_other [of 6 l xpc u8_list l1 "xpc1+3" reg]; simp?; linarith?)
+          done
+        done
+
+      apply ((erule case_option_eq_NE; simp?) | (erule ifE; erule conjE; simp))+
+      subgoal for reg src dst
+          apply (subst x64_bin_update_nth_error_other [of 6 l xpc u8_list l1 xpc1 h]; simp?; linarith?)
+          apply (rule conjI, rule impI)
+          subgoal by blast
+          apply (subst x64_bin_update_nth_error_other [of 6 l xpc u8_list l1 "xpc1+1" op]; simp?; linarith?)
+          apply (subst x64_bin_update_nth_error_other [of 6 l xpc u8_list l1 "xpc1+2" reg]; simp?; linarith?)
+          done
+        subgoal for reg
+          apply ((erule case_option_eq_NE; simp?) | (erule ifE; erule conjE; simp))+
+          subgoal for dis src dst
+            apply (subst x64_bin_update_nth_error_other [of 6 l xpc u8_list l1 xpc1 h]; simp?; linarith?)
+          apply (rule conjI, rule impI)
+          subgoal by blast
+            apply (subst x64_bin_update_nth_error_other [of 6 l xpc u8_list l1 "xpc1+1" op]; simp?; linarith?)
+            apply (subst x64_bin_update_nth_error_other [of 6 l xpc u8_list l1 "xpc1+2" reg]; simp?; linarith?)
+            apply (subst x64_bin_update_nth_error_other [of 6 l xpc u8_list l1 "xpc1+3" dis]; simp?; linarith?)
+            done
+
+          apply ((erule case_option_eq_NE; simp?) | (erule ifE; erule conjE; simp))+
+          subgoal for d1 d2 d3 d4 dis src rb
+            apply (subst x64_bin_update_nth_error_other [of 6 l xpc u8_list l1 xpc1 h]; simp?; linarith?)
+          apply (rule conjI, rule impI)
+          subgoal by blast
+            apply (subst x64_bin_update_nth_error_other [of 6 l xpc u8_list l1 "xpc1+1" op]; simp?; linarith?)
+            apply (subst x64_bin_update_nth_error_other [of 6 l xpc u8_list l1 "xpc1+2" reg]; simp?; linarith?)
+            apply (subst x64_bin_update_nth_error_other [of 6 l xpc u8_list l1 "xpc1+3" d1]; simp?; linarith?)
+            apply (subst x64_bin_update_nth_error_other [of 6 l xpc u8_list l1 "xpc1+4" d2]; simp?; linarith?)
+            apply (subst x64_bin_update_nth_error_other [of 6 l xpc u8_list l1 "xpc1+5" d3]; simp?; linarith?)
+            apply (subst x64_bin_update_nth_error_other [of 6 l xpc u8_list l1 "xpc1+6" d4]; simp?; linarith?)
+            done
+
+          apply ((erule case_option_eq_NE; simp?) | (erule ifE; erule conjE; simp))+
+          subgoal for sib d1 d2 d3 d4 dis src ri rb
+            apply (subst x64_bin_update_nth_error_other [of 6 l xpc u8_list l1 xpc1 h]; simp?; linarith?)
+          apply (rule conjI, rule impI)
+          subgoal by blast
+            apply (subst x64_bin_update_nth_error_other [of 6 l xpc u8_list l1 "xpc1+1" op]; simp?; linarith?)
+            apply (subst x64_bin_update_nth_error_other [of 6 l xpc u8_list l1 "xpc1+2" reg]; simp?; linarith?)
+            apply (subst x64_bin_update_nth_error_other [of 6 l xpc u8_list l1 "xpc1+3" sib]; simp?; linarith?)
+            apply (subst x64_bin_update_nth_error_other [of 6 l xpc u8_list l1 "xpc1+4" d1]; simp?; linarith?)
+            apply (subst x64_bin_update_nth_error_other [of 6 l xpc u8_list l1 "xpc1+5" d2]; simp?; linarith?)
+            apply (subst x64_bin_update_nth_error_other [of 6 l xpc u8_list l1 "xpc1+6" d3]; simp?; linarith?)
+            apply (subst x64_bin_update_nth_error_other [of 6 l xpc u8_list l1 "xpc1+7" d4]; simp?; linarith?)
+            done
+          done
+        subgoal for reg
+          apply ((erule case_option_eq_NE; simp?) | (erule ifE; erule conjE; simp))+
+          subgoal for src dst
+            apply (subst x64_bin_update_nth_error_other [of 6 l xpc u8_list l1 xpc1 h]; simp?; linarith?)
+          apply (rule conjI, rule impI)
+          subgoal by blast
+            apply (subst x64_bin_update_nth_error_other [of 6 l xpc u8_list l1 "xpc1+1" op]; simp?; linarith?)
+            apply (subst x64_bin_update_nth_error_other [of 6 l xpc u8_list l1 "xpc1+2" reg]; simp?; linarith?)
+            done
+
+          subgoal
+            apply ((erule case_option_eq_NE; simp?) | (erule ifE; erule conjE; simp))+
+            subgoal for sib d1 d2 d3 d4 dis src ri rb
+              apply (subst x64_bin_update_nth_error_other [of 6 l xpc u8_list l1 xpc1 h]; simp?; linarith?)
+          apply (rule conjI, rule impI)
+          subgoal by blast
+              apply (subst x64_bin_update_nth_error_other [of 6 l xpc u8_list l1 "xpc1+1" op]; simp?; linarith?)
+              apply (subst x64_bin_update_nth_error_other [of 6 l xpc u8_list l1 "xpc1+2" reg]; simp?; linarith?)
+              apply (subst x64_bin_update_nth_error_other [of 6 l xpc u8_list l1 "xpc1+3" sib]; simp?; linarith?)
+              apply (subst x64_bin_update_nth_error_other [of 6 l xpc u8_list l1 "xpc1+4" d1]; simp?; linarith?)
+              apply (subst x64_bin_update_nth_error_other [of 6 l xpc u8_list l1 "xpc1+5" d2]; simp?; linarith?)
+              apply (subst x64_bin_update_nth_error_other [of 6 l xpc u8_list l1 "xpc1+6" d3]; simp?; linarith?)
+              apply (subst x64_bin_update_nth_error_other [of 6 l xpc u8_list l1 "xpc1+7" d4]; simp?; linarith?)
+              done
+            done
+
+          apply ((erule case_option_eq_NE; simp?) | (erule ifE; erule conjE; simp))+
+          subgoal for src dst
+            apply (subst x64_bin_update_nth_error_other [of 6 l xpc u8_list l1 xpc1 h]; simp?; linarith?)
+          apply (rule conjI, rule impI)
+          subgoal by blast
+            apply (subst x64_bin_update_nth_error_other [of 6 l xpc u8_list l1 "xpc1+1" op]; simp?; linarith?)
+            apply (subst x64_bin_update_nth_error_other [of 6 l xpc u8_list l1 "xpc1+2" reg]; simp?; linarith?)
+            done
+
+          apply ((erule case_option_eq_NE; simp?) | (erule ifE; erule conjE; simp))+
+          subgoal for src dst
+            apply (subst x64_bin_update_nth_error_other [of 6 l xpc u8_list l1 xpc1 h]; simp?; linarith?)
+          apply (rule conjI, rule impI)
+          subgoal by blast
+            apply (subst x64_bin_update_nth_error_other [of 6 l xpc u8_list l1 "xpc1+1" op]; simp?; linarith?)
+            apply (subst x64_bin_update_nth_error_other [of 6 l xpc u8_list l1 "xpc1+2" reg]; simp?; linarith?)
+            done
+
+          apply ((erule case_option_eq_NE; simp?) | (erule ifE; erule conjE; simp))+
+          subgoal for src dst
+            apply (subst x64_bin_update_nth_error_other [of 6 l xpc u8_list l1 xpc1 h]; simp?; linarith?)
+          apply (rule conjI, rule impI)
+          subgoal by blast
+            apply (subst x64_bin_update_nth_error_other [of 6 l xpc u8_list l1 "xpc1+1" op]; simp?; linarith?)
+            apply (subst x64_bin_update_nth_error_other [of 6 l xpc u8_list l1 "xpc1+2" reg]; simp?; linarith?)
+            done
+
+          apply ((erule case_option_eq_NE; simp?) | (erule ifE; erule conjE; simp))+
+          subgoal for dst
+            apply (subst x64_bin_update_nth_error_other [of 6 l xpc u8_list l1 xpc1 h]; simp?; linarith?)
+            apply (subst x64_bin_update_nth_error_other [of 6 l xpc u8_list l1 "xpc1+1" op]; simp?; linarith?)
+            apply (subst x64_bin_update_nth_error_other [of 6 l xpc u8_list l1 "xpc1+2" reg]; simp?; linarith?)
+            done
+          subgoal
+            apply ((erule case_option_eq_NE; simp?) | (erule ifE; erule conjE; simp))+
+            subgoal for dst
+              apply (subst x64_bin_update_nth_error_other [of 6 l xpc u8_list l1 xpc1 h]; simp?; linarith?)
+              apply (subst x64_bin_update_nth_error_other [of 6 l xpc u8_list l1 "xpc1+1" op]; simp?; linarith?)
+              apply (subst x64_bin_update_nth_error_other [of 6 l xpc u8_list l1 "xpc1+2" reg]; simp?; linarith?)
+              done
+            apply ((erule case_option_eq_NE; simp?) | (erule ifE; erule conjE; simp))+
+            subgoal for dst
+              apply (subst x64_bin_update_nth_error_other [of 6 l xpc u8_list l1 xpc1 h]; simp?; linarith?)
+              apply (subst x64_bin_update_nth_error_other [of 6 l xpc u8_list l1 "xpc1+1" op]; simp?; linarith?)
+              apply (subst x64_bin_update_nth_error_other [of 6 l xpc u8_list l1 "xpc1+2" reg]; simp?; linarith?)
+              done
+
+
+            apply ((erule case_option_eq_NE; simp?) | (erule ifE; erule conjE; simp))+
+            subgoal for dst
+              apply (subst x64_bin_update_nth_error_other [of 6 l xpc u8_list l1 xpc1 h]; simp?; linarith?)
+              apply (subst x64_bin_update_nth_error_other [of 6 l xpc u8_list l1 "xpc1+1" op]; simp?; linarith?)
+              apply (subst x64_bin_update_nth_error_other [of 6 l xpc u8_list l1 "xpc1+2" reg]; simp?; linarith?)
+              done
+
+            apply ((erule case_option_eq_NE; simp?) | (erule ifE; erule conjE; simp))+
+            subgoal for dst
+              apply (subst x64_bin_update_nth_error_other [of 6 l xpc u8_list l1 xpc1 h]; simp?; linarith?)
+              apply (subst x64_bin_update_nth_error_other [of 6 l xpc u8_list l1 "xpc1+1" op]; simp?; linarith?)
+              apply (subst x64_bin_update_nth_error_other [of 6 l xpc u8_list l1 "xpc1+2" reg]; simp?; linarith?)
+              done
+
+            apply ((erule case_option_eq_NE; simp?) | (erule ifE; erule conjE; simp))+
+            subgoal for i1 i2 i3 i4 dst imm
+              apply (subst x64_bin_update_nth_error_other [of 6 l xpc u8_list l1 xpc1 h]; simp?; linarith?)
+              apply (subst x64_bin_update_nth_error_other [of 6 l xpc u8_list l1 "xpc1+1" op]; simp?; linarith?)
+              apply (subst x64_bin_update_nth_error_other [of 6 l xpc u8_list l1 "xpc1+2" reg]; simp?; linarith?)
+              apply (subst x64_bin_update_nth_error_other [of 6 l xpc u8_list l1 "xpc1+3" i1]; simp?; linarith?)
+              apply (subst x64_bin_update_nth_error_other [of 6 l xpc u8_list l1 "xpc1+4" i2]; simp?; linarith?)
+              apply (subst x64_bin_update_nth_error_other [of 6 l xpc u8_list l1 "xpc1+5" i3]; simp?; linarith?)
+              apply (subst x64_bin_update_nth_error_other [of 6 l xpc u8_list l1 "xpc1+6" i4]; simp?; linarith?)
+              done
+            done
+
+          apply ((erule case_option_eq_NE; simp?) | (erule ifE; erule conjE; simp))+
+          subgoal for src dst
+            apply (subst x64_bin_update_nth_error_other [of 6 l xpc u8_list l1 xpc1 h]; simp?; linarith?)
+          apply (rule conjI, rule impI)
+          subgoal by blast
+            apply (subst x64_bin_update_nth_error_other [of 6 l xpc u8_list l1 "xpc1+1" op]; simp?; linarith?)
+            apply (subst x64_bin_update_nth_error_other [of 6 l xpc u8_list l1 "xpc1+2" reg]; simp?; linarith?)
+            done
+
+          apply ((erule case_option_eq_NE; simp?) | (erule ifE; erule conjE; simp))+
+          subgoal for src dst
+            apply (subst x64_bin_update_nth_error_other [of 6 l xpc u8_list l1 xpc1 h]; simp?; linarith?)
+          apply (rule conjI, rule impI)
+          subgoal by blast
+            apply (subst x64_bin_update_nth_error_other [of 6 l xpc u8_list l1 "xpc1+1" op]; simp?; linarith?)
+            apply (subst x64_bin_update_nth_error_other [of 6 l xpc u8_list l1 "xpc1+2" reg]; simp?; linarith?)
+            done
+
+          apply ((erule case_option_eq_NE; simp?) | (erule ifE; erule conjE; simp))+
+          subgoal for src dst
+            apply (subst x64_bin_update_nth_error_other [of 6 l xpc u8_list l1 xpc1 h]; simp?; linarith?)
+          apply (rule conjI, rule impI)
+          subgoal by blast
+            apply (subst x64_bin_update_nth_error_other [of 6 l xpc u8_list l1 "xpc1+1" op]; simp?; linarith?)
+            apply (subst x64_bin_update_nth_error_other [of 6 l xpc u8_list l1 "xpc1+2" reg]; simp?; linarith?)
+            done
+
+          apply ((erule case_option_eq_NE; simp?) | (erule ifE; erule conjE; simp))+
+          subgoal for dst
+            apply (subst x64_bin_update_nth_error_other [of 6 l xpc u8_list l1 xpc1 h]; simp?; linarith?)
+            apply (subst x64_bin_update_nth_error_other [of 6 l xpc u8_list l1 "xpc1+1" op]; simp?; linarith?)
+            apply (subst x64_bin_update_nth_error_other [of 6 l xpc u8_list l1 "xpc1+2" reg]; simp?; linarith?)
+            done
+          subgoal
+            apply ((erule case_option_eq_NE; simp?) | (erule ifE; erule conjE; simp))+
+            subgoal for dst
+              apply (subst x64_bin_update_nth_error_other [of 6 l xpc u8_list l1 xpc1 h]; simp?; linarith?)
+              apply (subst x64_bin_update_nth_error_other [of 6 l xpc u8_list l1 "xpc1+1" op]; simp?; linarith?)
+              apply (subst x64_bin_update_nth_error_other [of 6 l xpc u8_list l1 "xpc1+2" reg]; simp?; linarith?)
+              done
+
+            apply ((erule case_option_eq_NE; simp?) | (erule ifE; erule conjE; simp))+
+            subgoal for dst
+              apply (subst x64_bin_update_nth_error_other [of 6 l xpc u8_list l1 xpc1 h]; simp?; linarith?)
+              apply (subst x64_bin_update_nth_error_other [of 6 l xpc u8_list l1 "xpc1+1" op]; simp?; linarith?)
+              apply (subst x64_bin_update_nth_error_other [of 6 l xpc u8_list l1 "xpc1+2" reg]; simp?; linarith?)
+              done
+            done
+          apply ((erule case_option_eq_NE; simp?) | (erule ifE; erule conjE; simp))+
+          subgoal for dst
+            apply (subst x64_bin_update_nth_error_other [of 6 l xpc u8_list l1 xpc1 h]; simp?; linarith?)
+          apply (rule conjI, rule impI)
+          subgoal by blast
+            apply (subst x64_bin_update_nth_error_other [of 6 l xpc u8_list l1 "xpc1+1" op]; simp?; linarith?)
+            apply (subst x64_bin_update_nth_error_other [of 6 l xpc u8_list l1 "xpc1+2" reg]; simp?; linarith?)
+            done
+
+          apply ((erule case_option_eq_NE; simp?) | (erule ifE; erule conjE; simp))+
+          subgoal for dst
+            apply (subst x64_bin_update_nth_error_other [of 6 l xpc u8_list l1 xpc1 h]; simp?; linarith?)
+          apply (rule conjI, rule impI)
+          subgoal by blast
+            apply (subst x64_bin_update_nth_error_other [of 6 l xpc u8_list l1 "xpc1+1" op]; simp?; linarith?)
+            apply (subst x64_bin_update_nth_error_other [of 6 l xpc u8_list l1 "xpc1+2" reg]; simp?; linarith?)
+            done
+
+          apply ((erule case_option_eq_NE; simp?) | (erule ifE; erule conjE; simp))+
+          subgoal for sib d1 d2 d3 d4 dis
+            apply (erule conjE)
+            apply ((erule case_option_eq_NE; simp?) | (erule ifE; erule conjE; simp))+
+            subgoal for ri rb
+              apply (subst x64_bin_update_nth_error_other [of 6 l xpc u8_list l1 xpc1 h]; simp?; linarith?)
+          apply (rule conjI, rule impI)
+          subgoal by blast
+              apply (subst x64_bin_update_nth_error_other [of 6 l xpc u8_list l1 "xpc1+1" op]; simp?; linarith?)
+              apply (subst x64_bin_update_nth_error_other [of 6 l xpc u8_list l1 "xpc1+2" reg]; simp?; linarith?)
+              apply (subst x64_bin_update_nth_error_other [of 6 l xpc u8_list l1 "xpc1+3" sib]; simp?; linarith?)
+              apply (subst x64_bin_update_nth_error_other [of 6 l xpc u8_list l1 "xpc1+4" d1]; simp?; linarith?)
+              apply (subst x64_bin_update_nth_error_other [of 6 l xpc u8_list l1 "xpc1+5" d2]; simp?; linarith?)
+              apply (subst x64_bin_update_nth_error_other [of 6 l xpc u8_list l1 "xpc1+6" d3]; simp?; linarith?)
+              apply (subst x64_bin_update_nth_error_other [of 6 l xpc u8_list l1 "xpc1+7" d4]; simp?; linarith?)
+              done
+            done
+
+          apply ((erule case_option_eq_NE; simp?) | (erule ifE; erule conjE; simp))+
+          subgoal for i1 i2 i3 i4 dst imm
+            apply (erule conjE)+
+            apply ((erule case_option_eq_NE; simp?) | (erule ifE; erule conjE; simp))+
+            subgoal for dis
+              apply (subst x64_bin_update_nth_error_other [of 6 l xpc u8_list l1 xpc1 h]; simp?; linarith?)
+              apply (subst x64_bin_update_nth_error_other [of 6 l xpc u8_list l1 "xpc1+1" op]; simp?; linarith?)
+              apply (subst x64_bin_update_nth_error_other [of 6 l xpc u8_list l1 "xpc1+2" reg]; simp?; linarith?)
+              apply (subst x64_bin_update_nth_error_other [of 6 l xpc u8_list l1 "4+xpc1" i1]; simp?; linarith?)
+              apply (subst x64_bin_update_nth_error_other [of 6 l xpc u8_list l1 "5+xpc1" i2]; simp?; linarith?)
+              apply (subst x64_bin_update_nth_error_other [of 6 l xpc u8_list l1 "6+xpc1" i3]; simp?; linarith?)
+              apply (subst x64_bin_update_nth_error_other [of 6 l xpc u8_list l1 "7+xpc1" i4]; simp?; linarith?)
+              apply (subst x64_bin_update_nth_error_other [of 6 l xpc u8_list l1 "xpc1+3" dis]; simp?; linarith?)
+              done
+            subgoal
+              apply ((erule case_option_eq_NE; simp?) | (erule ifE; erule conjE; simp))+
+              subgoal for d1 d2 d3 d4 dis
+                apply (subst x64_bin_update_nth_error_other [of 6 l xpc u8_list l1 xpc1 h]; simp?; linarith?)
+                apply (subst x64_bin_update_nth_error_other [of 6 l xpc u8_list l1 "xpc1+1" op]; simp?; linarith?)
+                apply (subst x64_bin_update_nth_error_other [of 6 l xpc u8_list l1 "xpc1+2" reg]; simp?; linarith?)
+                apply (subst x64_bin_update_nth_error_other [of 6 l xpc u8_list l1 "7+xpc1" i1]; simp?; linarith?)
+                apply (subst x64_bin_update_nth_error_other [of 6 l xpc u8_list l1 "8+xpc1" i2]; simp?; linarith?)
+                apply (subst x64_bin_update_nth_error_other [of 6 l xpc u8_list l1 "9+xpc1" i3]; simp?; linarith?)
+                apply (subst x64_bin_update_nth_error_other [of 6 l xpc u8_list l1 "10+xpc1" i4]; simp?; linarith?)
+                apply (subst x64_bin_update_nth_error_other [of 6 l xpc u8_list l1 "xpc1+3" d1]; simp?; linarith?)
+                apply (subst x64_bin_update_nth_error_other [of 6 l xpc u8_list l1 "xpc1+4" d2]; simp?; linarith?)
+                apply (subst x64_bin_update_nth_error_other [of 6 l xpc u8_list l1 "xpc1+5" d3]; simp?; linarith?)
+                apply (subst x64_bin_update_nth_error_other [of 6 l xpc u8_list l1 "xpc1+6" d4]; simp?; linarith?)
+                done
+              done
+            done
+
+          apply ((erule case_option_eq_NE; simp?) | (erule ifE; erule conjE; simp))+
+          subgoal for dst i1 i2 i3 i4 imm
+            apply (subst x64_bin_update_nth_error_other [of 6 l xpc u8_list l1 xpc1 h]; simp?; linarith?)
+            apply (subst x64_bin_update_nth_error_other [of 6 l xpc u8_list l1 "xpc1+1" op]; simp?; linarith?)
+            apply (subst x64_bin_update_nth_error_other [of 6 l xpc u8_list l1 "xpc1+2" reg]; simp?; linarith?)
+            apply (subst x64_bin_update_nth_error_other [of 6 l xpc u8_list l1 "xpc1+3" i1]; simp?; linarith?)
+            apply (subst x64_bin_update_nth_error_other [of 6 l xpc u8_list l1 "xpc1+4" i2]; simp?; linarith?)
+            apply (subst x64_bin_update_nth_error_other [of 6 l xpc u8_list l1 "xpc1+5" i3]; simp?; linarith?)
+            apply (subst x64_bin_update_nth_error_other [of 6 l xpc u8_list l1 "xpc1+6" i4]; simp?; linarith?)
+            done
+
+           apply ((erule case_option_eq_NE; simp?) | (erule ifE; erule conjE; simp))+
+          subgoal for sib d1 d2 d3 d4 dis
+            apply (erule conjE)
+            apply ((erule case_option_eq_NE; simp?) | (erule ifE; erule conjE; simp))+
+            subgoal for i1 i2 i3 i4 imm ri rb
+              apply (subst x64_bin_update_nth_error_other [of 6 l xpc u8_list l1 xpc1 h]; simp?; linarith?)
+          apply (rule conjI, rule impI)
+          subgoal by blast
+              apply (subst x64_bin_update_nth_error_other [of 6 l xpc u8_list l1 "xpc1+1" op]; simp?; linarith?)
+              apply (subst x64_bin_update_nth_error_other [of 6 l xpc u8_list l1 "xpc1+2" reg]; simp?; linarith?)
+              apply (subst x64_bin_update_nth_error_other [of 6 l xpc u8_list l1 "xpc1+3" sib]; simp?; linarith?)
+              apply (subst x64_bin_update_nth_error_other [of 6 l xpc u8_list l1 "xpc1+4" d1]; simp?; linarith?)
+              apply (subst x64_bin_update_nth_error_other [of 6 l xpc u8_list l1 "xpc1+5" d2]; simp?; linarith?)
+              apply (subst x64_bin_update_nth_error_other [of 6 l xpc u8_list l1 "xpc1+6" d3]; simp?; linarith?)
+              apply (subst x64_bin_update_nth_error_other [of 6 l xpc u8_list l1 "xpc1+7" d4]; simp?; linarith?)
+              apply (subst x64_bin_update_nth_error_other [of 6 l xpc u8_list l1 "xpc1+8" i1]; simp?; linarith?)
+              apply (subst x64_bin_update_nth_error_other [of 6 l xpc u8_list l1 "xpc1+9" i2]; simp?; linarith?)
+              apply (subst x64_bin_update_nth_error_other [of 6 l xpc u8_list l1 "xpc1+10" i3]; simp?; linarith?)
+              apply (subst x64_bin_update_nth_error_other [of 6 l xpc u8_list l1 "xpc1+11" i4]; simp?; linarith?)
+              done
+            done
+
+          apply ((erule case_option_eq_NE; simp?) | (erule ifE; erule conjE; simp))+
+          subgoal for imm dst
+            apply (subst x64_bin_update_nth_error_other [of 6 l xpc u8_list l1 xpc1 h]; simp?; linarith?)
+            apply (subst x64_bin_update_nth_error_other [of 6 l xpc u8_list l1 "xpc1+1" op]; simp?; linarith?)
+            apply (subst x64_bin_update_nth_error_other [of 6 l xpc u8_list l1 "xpc1+2" reg]; simp?; linarith?)
+            apply (subst x64_bin_update_nth_error_other [of 6 l xpc u8_list l1 "xpc1+3" imm]; simp?; linarith?)
+            done
+
+          subgoal for imm
+            apply ((erule case_option_eq_NE; simp?) | (erule ifE; erule conjE; simp))+
+            subgoal for dst
+              apply (subst x64_bin_update_nth_error_other [of 6 l xpc u8_list l1 xpc1 h]; simp?; linarith?)
+              apply (subst x64_bin_update_nth_error_other [of 6 l xpc u8_list l1 "xpc1+1" op]; simp?; linarith?)
+              apply (subst x64_bin_update_nth_error_other [of 6 l xpc u8_list l1 "xpc1+2" reg]; simp?; linarith?)
+              apply (subst x64_bin_update_nth_error_other [of 6 l xpc u8_list l1 "xpc1+3" imm]; simp?; linarith?)
+              done
+            apply ((erule case_option_eq_NE; simp?) | (erule ifE; erule conjE; simp))+
+            subgoal for dst
+              apply (subst x64_bin_update_nth_error_other [of 6 l xpc u8_list l1 xpc1 h]; simp?; linarith?)
+              apply (subst x64_bin_update_nth_error_other [of 6 l xpc u8_list l1 "xpc1+1" op]; simp?; linarith?)
+              apply (subst x64_bin_update_nth_error_other [of 6 l xpc u8_list l1 "xpc1+2" reg]; simp?; linarith?)
+              apply (subst x64_bin_update_nth_error_other [of 6 l xpc u8_list l1 "xpc1+3" imm]; simp?; linarith?)
+              done
+            done
+
+          apply ((erule case_option_eq_NE; simp?) | (erule ifE; erule conjE; simp))+
+          subgoal for dis src dst
+            apply (subst x64_bin_update_nth_error_other [of 6 l xpc u8_list l1 xpc1 h]; simp?; linarith?)
+          apply (rule conjI, rule impI)
+          subgoal by blast
+            apply (subst x64_bin_update_nth_error_other [of 6 l xpc u8_list l1 "xpc1+1" op]; simp?; linarith?)
+            apply (subst x64_bin_update_nth_error_other [of 6 l xpc u8_list l1 "xpc1+2" reg]; simp?; linarith?)
+            apply (subst x64_bin_update_nth_error_other [of 6 l xpc u8_list l1 "xpc1+3" dis]; simp?; linarith?)
+            done
+          subgoal 
+            apply ((erule case_option_eq_NE; simp?) | (erule ifE; erule conjE; simp))+
+            subgoal for d1 d2 d3 d4 dis src dst
+              apply (subst x64_bin_update_nth_error_other [of 6 l xpc u8_list l1 xpc1 h]; simp?; linarith?)
+          apply (rule conjI, rule impI)
+          subgoal by blast
+              apply (subst x64_bin_update_nth_error_other [of 6 l xpc u8_list l1 "xpc1+1" op]; simp?; linarith?)
+              apply (subst x64_bin_update_nth_error_other [of 6 l xpc u8_list l1 "xpc1+2" reg]; simp?; linarith?)
+              apply (subst x64_bin_update_nth_error_other [of 6 l xpc u8_list l1 "xpc1+3" d1]; simp?; linarith?)
+              apply (subst x64_bin_update_nth_error_other [of 6 l xpc u8_list l1 "xpc1+4" d2]; simp?; linarith?)
+              apply (subst x64_bin_update_nth_error_other [of 6 l xpc u8_list l1 "xpc1+5" d3]; simp?; linarith?)
+              apply (subst x64_bin_update_nth_error_other [of 6 l xpc u8_list l1 "xpc1+6" d4]; simp?; linarith?)
+              done
+
+            apply ((erule case_option_eq_NE; simp?) | (erule ifE; erule conjE; simp))+
+            subgoal for sib d1 d2 d3 d4 dis src ri rb
+              apply (subst x64_bin_update_nth_error_other [of 6 l xpc u8_list l1 xpc1 h]; simp?; linarith?)
+          apply (rule conjI, rule impI)
+          subgoal by blast
+              apply (subst x64_bin_update_nth_error_other [of 6 l xpc u8_list l1 "xpc1+1" op]; simp?; linarith?)
+              apply (subst x64_bin_update_nth_error_other [of 6 l xpc u8_list l1 "xpc1+2" reg]; simp?; linarith?)
+              apply (subst x64_bin_update_nth_error_other [of 6 l xpc u8_list l1 "xpc1+3" sib]; simp?; linarith?)
+              apply (subst x64_bin_update_nth_error_other [of 6 l xpc u8_list l1 "xpc1+4" d1]; simp?; linarith?)
+              apply (subst x64_bin_update_nth_error_other [of 6 l xpc u8_list l1 "xpc1+5" d2]; simp?; linarith?)
+              apply (subst x64_bin_update_nth_error_other [of 6 l xpc u8_list l1 "xpc1+6" d3]; simp?; linarith?)
+              apply (subst x64_bin_update_nth_error_other [of 6 l xpc u8_list l1 "xpc1+7" d4]; simp?; linarith?)
+              done
+            done
+
+          apply ((erule case_option_eq_NE; simp?) | (erule ifE; erule conjE; simp))+
+          subgoal for dis src dst
+            apply (subst x64_bin_update_nth_error_other [of 6 l xpc u8_list l1 xpc1 h]; simp?; linarith?)
+          apply (rule conjI, rule impI)
+          subgoal by blast
+            apply (subst x64_bin_update_nth_error_other [of 6 l xpc u8_list l1 "xpc1+1" op]; simp?; linarith?)
+            apply (subst x64_bin_update_nth_error_other [of 6 l xpc u8_list l1 "xpc1+2" reg]; simp?; linarith?)
+            apply (subst x64_bin_update_nth_error_other [of 6 l xpc u8_list l1 "xpc1+3" dis]; simp?; linarith?)
+            done
+          subgoal
+            apply ((erule case_option_eq_NE; simp?) | (erule ifE; erule conjE; simp))+
+            subgoal for d1 d2 d3 d4 dis src dst
+              apply (subst x64_bin_update_nth_error_other [of 6 l xpc u8_list l1 xpc1 h]; simp?; linarith?)
+          apply (rule conjI, rule impI)
+          subgoal by blast
+              apply (subst x64_bin_update_nth_error_other [of 6 l xpc u8_list l1 "xpc1+1" op]; simp?; linarith?)
+              apply (subst x64_bin_update_nth_error_other [of 6 l xpc u8_list l1 "xpc1+2" reg]; simp?; linarith?)
+              apply (subst x64_bin_update_nth_error_other [of 6 l xpc u8_list l1 "xpc1+3" d1]; simp?; linarith?)
+              apply (subst x64_bin_update_nth_error_other [of 6 l xpc u8_list l1 "xpc1+4" d2]; simp?; linarith?)
+              apply (subst x64_bin_update_nth_error_other [of 6 l xpc u8_list l1 "xpc1+5" d3]; simp?; linarith?)
+              apply (subst x64_bin_update_nth_error_other [of 6 l xpc u8_list l1 "xpc1+6" d4]; simp?; linarith?)
+              done
+            done
+          done
+        done
+      done
+
+
+
+  subgoal for h
+    apply ((erule case_option_eq_NE; simp?) | (erule ifE; erule conjE; simp))+
+    subgoal for op dst
+      apply (subst x64_bin_update_nth_error_other [of 6 l xpc u8_list l1 xpc1 h]; simp?; linarith?)
+      apply (subst x64_bin_update_nth_error_other [of 6 l xpc u8_list l1 "xpc1+1" op]; simp?; linarith?)
+      done
+    subgoal for op
+      apply ((erule case_option_eq_NE; simp?) | (erule ifE; erule conjE; simp))+
+      subgoal for dst
+        apply (subst x64_bin_update_nth_error_other [of 6 l xpc u8_list l1 xpc1 h]; simp?; linarith?)
+        apply (subst x64_bin_update_nth_error_other [of 6 l xpc u8_list l1 "xpc1+1" op]; simp?; linarith?)
+        done
+      subgoal
+        apply ((erule case_option_eq_NE; simp?) | (erule ifE; erule conjE; simp))+
+        subgoal for op1 dst
+          apply (subst x64_bin_update_nth_error_other [of 6 l xpc u8_list l1 xpc1 h]; simp?; linarith?)
+          apply (subst x64_bin_update_nth_error_other [of 6 l xpc u8_list l1 "xpc1+1" op]; simp?; linarith?)
+          apply (subst x64_bin_update_nth_error_other [of 6 l xpc u8_list l1 "xpc1+2" op1]; simp?; linarith?)
+          done
+        subgoal for op1
+          apply ((erule case_option_eq_NE; simp?) | (erule ifE; erule conjE; simp))+
+          subgoal for reg t src dst
+          apply (subst x64_bin_update_nth_error_other [of 6 l xpc u8_list l1 xpc1 h]; simp?; linarith?)
+          apply (subst x64_bin_update_nth_error_other [of 6 l xpc u8_list l1 "xpc1+1" op]; simp?; linarith?)
+          apply (subst x64_bin_update_nth_error_other [of 6 l xpc u8_list l1 "xpc1+2" op1]; simp?; linarith?)
+          apply (subst x64_bin_update_nth_error_other [of 6 l xpc u8_list l1 "xpc1+3" reg]; simp?; linarith?)
+          done
+        done
+
+      apply ((erule case_option_eq_NE; simp?) | (erule ifE; erule conjE; simp))+
+      subgoal for reg src dst
+          apply (subst x64_bin_update_nth_error_other [of 6 l xpc u8_list l1 xpc1 h]; simp?; linarith?)
+          apply (subst x64_bin_update_nth_error_other [of 6 l xpc u8_list l1 "xpc1+1" op]; simp?; linarith?)
+          apply (subst x64_bin_update_nth_error_other [of 6 l xpc u8_list l1 "xpc1+2" reg]; simp?; linarith?)
+          done
+        subgoal for reg
+          apply ((erule case_option_eq_NE; simp?) | (erule ifE; erule conjE; simp))+
+          subgoal for dis src dst
+            apply (subst x64_bin_update_nth_error_other [of 6 l xpc u8_list l1 xpc1 h]; simp?; linarith?)
+            apply (subst x64_bin_update_nth_error_other [of 6 l xpc u8_list l1 "xpc1+1" op]; simp?; linarith?)
+            apply (subst x64_bin_update_nth_error_other [of 6 l xpc u8_list l1 "xpc1+2" reg]; simp?; linarith?)
+            apply (subst x64_bin_update_nth_error_other [of 6 l xpc u8_list l1 "xpc1+3" dis]; simp?; linarith?)
+            done
+
+          apply ((erule case_option_eq_NE; simp?) | (erule ifE; erule conjE; simp))+
+          subgoal for d1 d2 d3 d4 dis src rb
+            apply (subst x64_bin_update_nth_error_other [of 6 l xpc u8_list l1 xpc1 h]; simp?; linarith?)
+            apply (subst x64_bin_update_nth_error_other [of 6 l xpc u8_list l1 "xpc1+1" op]; simp?; linarith?)
+            apply (subst x64_bin_update_nth_error_other [of 6 l xpc u8_list l1 "xpc1+2" reg]; simp?; linarith?)
+            apply (subst x64_bin_update_nth_error_other [of 6 l xpc u8_list l1 "xpc1+3" d1]; simp?; linarith?)
+            apply (subst x64_bin_update_nth_error_other [of 6 l xpc u8_list l1 "xpc1+4" d2]; simp?; linarith?)
+            apply (subst x64_bin_update_nth_error_other [of 6 l xpc u8_list l1 "xpc1+5" d3]; simp?; linarith?)
+            apply (subst x64_bin_update_nth_error_other [of 6 l xpc u8_list l1 "xpc1+6" d4]; simp?; linarith?)
+            done
+
+          apply ((erule case_option_eq_NE; simp?) | (erule ifE; erule conjE; simp))+
+          done
+        subgoal for reg
+          apply ((erule case_option_eq_NE; simp?) | (erule ifE; erule conjE; simp))+
+          subgoal for src dst
+            apply (subst x64_bin_update_nth_error_other [of 6 l xpc u8_list l1 xpc1 h]; simp?; linarith?)
+            apply (subst x64_bin_update_nth_error_other [of 6 l xpc u8_list l1 "xpc1+1" op]; simp?; linarith?)
+            apply (subst x64_bin_update_nth_error_other [of 6 l xpc u8_list l1 "xpc1+2" reg]; simp?; linarith?)
+            done
+
+          subgoal
+            apply ((erule case_option_eq_NE; simp?) | (erule ifE; erule conjE; simp))+
+            subgoal for src dst
+              apply (subst x64_bin_update_nth_error_other [of 6 l xpc u8_list l1 xpc1 h]; simp?; linarith?)
+              apply (subst x64_bin_update_nth_error_other [of 6 l xpc u8_list l1 "xpc1+1" op]; simp?; linarith?)
+              apply (subst x64_bin_update_nth_error_other [of 6 l xpc u8_list l1 "xpc1+2" reg]; simp?; linarith?)
+              done
+
+            apply ((erule case_option_eq_NE; simp?) | (erule ifE; erule conjE; simp))+
+            subgoal for dst
+              apply (subst x64_bin_update_nth_error_other [of 6 l xpc u8_list l1 xpc1 h]; simp?; linarith?)
+              apply (subst x64_bin_update_nth_error_other [of 6 l xpc u8_list l1 "xpc1+1" op]; simp?; linarith?)
+              apply (subst x64_bin_update_nth_error_other [of 6 l xpc u8_list l1 "xpc1+2" reg]; simp?; linarith?)
+              done
+            subgoal
+              apply ((erule case_option_eq_NE; simp?) | (erule ifE; erule conjE; simp))+
+              subgoal for dst
+                apply (subst x64_bin_update_nth_error_other [of 6 l xpc u8_list l1 xpc1 h]; simp?; linarith?)
+                apply (subst x64_bin_update_nth_error_other [of 6 l xpc u8_list l1 "xpc1+1" op]; simp?; linarith?)
+                apply (subst x64_bin_update_nth_error_other [of 6 l xpc u8_list l1 "xpc1+2" reg]; simp?; linarith?)
+                done
+              apply ((erule case_option_eq_NE; simp?) | (erule ifE; erule conjE; simp))+
+              subgoal for dst
+                apply (subst x64_bin_update_nth_error_other [of 6 l xpc u8_list l1 xpc1 h]; simp?; linarith?)
+                apply (subst x64_bin_update_nth_error_other [of 6 l xpc u8_list l1 "xpc1+1" op]; simp?; linarith?)
+                apply (subst x64_bin_update_nth_error_other [of 6 l xpc u8_list l1 "xpc1+2" reg]; simp?; linarith?)
+                done
+              apply ((erule case_option_eq_NE; simp?) | (erule ifE; erule conjE; simp))+
+              subgoal for dst
+                apply (subst x64_bin_update_nth_error_other [of 6 l xpc u8_list l1 xpc1 h]; simp?; linarith?)
+                apply (subst x64_bin_update_nth_error_other [of 6 l xpc u8_list l1 "xpc1+1" op]; simp?; linarith?)
+                apply (subst x64_bin_update_nth_error_other [of 6 l xpc u8_list l1 "xpc1+2" reg]; simp?; linarith?)
+                done
+              apply ((erule case_option_eq_NE; simp?) | (erule ifE; erule conjE; simp))+
+              subgoal for dst
+                apply (subst x64_bin_update_nth_error_other [of 6 l xpc u8_list l1 xpc1 h]; simp?; linarith?)
+                apply (subst x64_bin_update_nth_error_other [of 6 l xpc u8_list l1 "xpc1+1" op]; simp?; linarith?)
+                apply (subst x64_bin_update_nth_error_other [of 6 l xpc u8_list l1 "xpc1+2" reg]; simp?; linarith?)
+                done
+              apply ((erule case_option_eq_NE; simp?) | (erule ifE; erule conjE; simp))+
+              subgoal for i1 i2 i3 i4 dst imm
+                apply (subst x64_bin_update_nth_error_other [of 6 l xpc u8_list l1 xpc1 h]; simp?; linarith?)
+                apply (subst x64_bin_update_nth_error_other [of 6 l xpc u8_list l1 "xpc1+1" op]; simp?; linarith?)
+                apply (subst x64_bin_update_nth_error_other [of 6 l xpc u8_list l1 "xpc1+2" reg]; simp?; linarith?)
+                apply (subst x64_bin_update_nth_error_other [of 6 l xpc u8_list l1 "xpc1+3" i1]; simp?; linarith?)
+                apply (subst x64_bin_update_nth_error_other [of 6 l xpc u8_list l1 "xpc1+4" i2]; simp?; linarith?)
+                apply (subst x64_bin_update_nth_error_other [of 6 l xpc u8_list l1 "xpc1+5" i3]; simp?; linarith?)
+                apply (subst x64_bin_update_nth_error_other [of 6 l xpc u8_list l1 "xpc1+6" i4]; simp?; linarith?)
+                done
+              done
+
+            apply ((erule case_option_eq_NE; simp?) | (erule ifE; erule conjE; simp))+
+            subgoal for src dst
+              apply (subst x64_bin_update_nth_error_other [of 6 l xpc u8_list l1 xpc1 h]; simp?; linarith?)
+              apply (subst x64_bin_update_nth_error_other [of 6 l xpc u8_list l1 "xpc1+1" op]; simp?; linarith?)
+              apply (subst x64_bin_update_nth_error_other [of 6 l xpc u8_list l1 "xpc1+2" reg]; simp?; linarith?)
+              done
+
+            apply ((erule case_option_eq_NE; simp?) | (erule ifE; erule conjE; simp))+
+            subgoal for src dst
+              apply (subst x64_bin_update_nth_error_other [of 6 l xpc u8_list l1 xpc1 h]; simp?; linarith?)
+              apply (subst x64_bin_update_nth_error_other [of 6 l xpc u8_list l1 "xpc1+1" op]; simp?; linarith?)
+              apply (subst x64_bin_update_nth_error_other [of 6 l xpc u8_list l1 "xpc1+2" reg]; simp?; linarith?)
+              done
+
+            apply ((erule case_option_eq_NE; simp?) | (erule ifE; erule conjE; simp))+
+            subgoal for src dst
+              apply (subst x64_bin_update_nth_error_other [of 6 l xpc u8_list l1 xpc1 h]; simp?; linarith?)
+              apply (subst x64_bin_update_nth_error_other [of 6 l xpc u8_list l1 "xpc1+1" op]; simp?; linarith?)
+              apply (subst x64_bin_update_nth_error_other [of 6 l xpc u8_list l1 "xpc1+2" reg]; simp?; linarith?)
+              done
+
+            apply ((erule case_option_eq_NE; simp?) | (erule ifE; erule conjE; simp))+
+            subgoal for dst
+              apply (subst x64_bin_update_nth_error_other [of 6 l xpc u8_list l1 xpc1 h]; simp?; linarith?)
+              apply (subst x64_bin_update_nth_error_other [of 6 l xpc u8_list l1 "xpc1+1" op]; simp?; linarith?)
+              apply (subst x64_bin_update_nth_error_other [of 6 l xpc u8_list l1 "xpc1+2" reg]; simp?; linarith?)
+              done
+            subgoal
+              apply ((erule case_option_eq_NE; simp?) | (erule ifE; erule conjE; simp))+
+              subgoal for dst
+                apply (subst x64_bin_update_nth_error_other [of 6 l xpc u8_list l1 xpc1 h]; simp?; linarith?)
+                apply (subst x64_bin_update_nth_error_other [of 6 l xpc u8_list l1 "xpc1+1" op]; simp?; linarith?)
+                apply (subst x64_bin_update_nth_error_other [of 6 l xpc u8_list l1 "xpc1+2" reg]; simp?; linarith?)
+                done
+
+              apply ((erule case_option_eq_NE; simp?) | (erule ifE; erule conjE; simp))+
+              subgoal for dst
+                apply (subst x64_bin_update_nth_error_other [of 6 l xpc u8_list l1 xpc1 h]; simp?; linarith?)
+                apply (subst x64_bin_update_nth_error_other [of 6 l xpc u8_list l1 "xpc1+1" op]; simp?; linarith?)
+                apply (subst x64_bin_update_nth_error_other [of 6 l xpc u8_list l1 "xpc1+2" reg]; simp?; linarith?)
+                done
+              done
+            apply ((erule case_option_eq_NE; simp?) | (erule ifE; erule conjE; simp))+
+            subgoal for src dst
+              apply (subst x64_bin_update_nth_error_other [of 6 l xpc u8_list l1 xpc1 h]; simp?; linarith?)
+              apply (subst x64_bin_update_nth_error_other [of 6 l xpc u8_list l1 "xpc1+1" op]; simp?; linarith?)
+              apply (subst x64_bin_update_nth_error_other [of 6 l xpc u8_list l1 "xpc1+2" reg]; simp?; linarith?)
+              done
+
+            apply ((erule case_option_eq_NE; simp?) | (erule ifE; erule conjE; simp))+
+            subgoal for dst
+              apply (subst x64_bin_update_nth_error_other [of 6 l xpc u8_list l1 xpc1 h]; simp?; linarith?)
+              apply (subst x64_bin_update_nth_error_other [of 6 l xpc u8_list l1 "xpc1+1" op]; simp?; linarith?)
+              apply (subst x64_bin_update_nth_error_other [of 6 l xpc u8_list l1 "xpc1+2" reg]; simp?; linarith?)
+              done
+
+            apply ((erule case_option_eq_NE; simp?) | (erule ifE; erule conjE; simp))+
+            subgoal for dst
+              apply (subst x64_bin_update_nth_error_other [of 6 l xpc u8_list l1 xpc1 h]; simp?; linarith?)
+              apply (subst x64_bin_update_nth_error_other [of 6 l xpc u8_list l1 "xpc1+1" op]; simp?; linarith?)
+              apply (subst x64_bin_update_nth_error_other [of 6 l xpc u8_list l1 "xpc1+2" reg]; simp?; linarith?)
+              done
+
+            apply ((erule case_option_eq_NE; simp?) | (erule ifE; erule conjE; simp))+
+            subgoal for i1 i2 i3 i4 dst imm
+              apply (erule conjE)+
+              apply ((erule case_option_eq_NE; simp?) | (erule ifE; erule conjE; simp))+
+                apply (subst x64_bin_update_nth_error_other [of 6 l xpc u8_list l1 xpc1 h]; simp?; linarith?)
+                apply (subst x64_bin_update_nth_error_other [of 6 l xpc u8_list l1 "xpc1+1" op]; simp?; linarith?)
+                apply (subst x64_bin_update_nth_error_other [of 6 l xpc u8_list l1 "xpc1+2" reg]; simp?; linarith?)
+              apply (erule conjE)+
+              apply (subgoal_tac "nth_error l1 (xpc1 + 3) = Some i1"; simp?)
+               prefer 2
+              subgoal
+                apply (subst x64_bin_update_nth_error_other [of 6 l xpc u8_list l1 "xpc1+3" i1]; simp?; linarith?)
+                done
+              apply (subgoal_tac "nth_error l1 (xpc1 + 4) = Some i2"; simp?)
+               prefer 2
+              subgoal
+                apply (subst x64_bin_update_nth_error_other [of 6 l xpc u8_list l1 "xpc1+4" i2]; simp?; linarith?)
+                done
+              apply (subgoal_tac "nth_error l1 (xpc1 + 5) = Some i3"; simp?)
+               prefer 2
+              subgoal
+                apply (subst x64_bin_update_nth_error_other [of 6 l xpc u8_list l1 "xpc1+5" i3]; simp?; linarith?)
+                done
+              apply (subgoal_tac "nth_error l1 (xpc1 + 6) = Some i4"; simp?)
+              subgoal
+                apply (subst x64_bin_update_nth_error_other [of 6 l xpc u8_list l1 "xpc1+6" i4]; simp?; linarith?)
+                done
+              done
+            subgoal for i1 i2 i3 i4 dst imm
+              apply (erule conjE)+
+              apply ((erule case_option_eq_NE; simp?) | (erule ifE; erule conjE; simp))+
+              done
+
+            apply ((erule case_option_eq_NE; simp?) | (erule ifE; erule conjE; simp))+
+            subgoal for dst i1 i2 i3 i4 imm
+              apply (subst x64_bin_update_nth_error_other [of 6 l xpc u8_list l1 xpc1 h]; simp?; linarith?)
+              apply (subst x64_bin_update_nth_error_other [of 6 l xpc u8_list l1 "xpc1+1" op]; simp?; linarith?)
+              apply (subst x64_bin_update_nth_error_other [of 6 l xpc u8_list l1 "xpc1+2" reg]; simp?; linarith?)
+              apply (subst x64_bin_update_nth_error_other [of 6 l xpc u8_list l1 "xpc1+3" i1]; simp?; linarith?)
+              apply (subst x64_bin_update_nth_error_other [of 6 l xpc u8_list l1 "xpc1+4" i2]; simp?; linarith?)
+              apply (subst x64_bin_update_nth_error_other [of 6 l xpc u8_list l1 "xpc1+5" i3]; simp?; linarith?)
+              apply (subst x64_bin_update_nth_error_other [of 6 l xpc u8_list l1 "xpc1+6" i4]; simp?; linarith?)
+              done
+
+            apply ((erule case_option_eq_NE; simp?) | (erule ifE; erule conjE; simp))+
+            subgoal for dst i1 i2 i3 i4 imm
+              apply (subst x64_bin_update_nth_error_other [of 6 l xpc u8_list l1 xpc1 h]; simp?; linarith?)
+              apply (subst x64_bin_update_nth_error_other [of 6 l xpc u8_list l1 "xpc1+1" op]; simp?; linarith?)
+              apply (subst x64_bin_update_nth_error_other [of 6 l xpc u8_list l1 "xpc1+2" reg]; simp?; linarith?)
+              apply (subst x64_bin_update_nth_error_other [of 6 l xpc u8_list l1 "xpc1+3" i1]; simp?; linarith?)
+              apply (subst x64_bin_update_nth_error_other [of 6 l xpc u8_list l1 "xpc1+4" i2]; simp?; linarith?)
+              apply (subst x64_bin_update_nth_error_other [of 6 l xpc u8_list l1 "xpc1+5" i3]; simp?; linarith?)
+              apply (subst x64_bin_update_nth_error_other [of 6 l xpc u8_list l1 "xpc1+6" i4]; simp?; linarith?)
+              done
+
+            apply ((erule case_option_eq_NE; simp?) | (erule ifE; erule conjE; simp))+
+            subgoal for dst i1 i2 i3 i4 imm
+              apply (subst x64_bin_update_nth_error_other [of 6 l xpc u8_list l1 xpc1 h]; simp?; linarith?)
+              apply (subst x64_bin_update_nth_error_other [of 6 l xpc u8_list l1 "xpc1+1" op]; simp?; linarith?)
+              apply (subst x64_bin_update_nth_error_other [of 6 l xpc u8_list l1 "xpc1+2" reg]; simp?; linarith?)
+              apply (subst x64_bin_update_nth_error_other [of 6 l xpc u8_list l1 "xpc1+3" i1]; simp?; linarith?)
+              apply (subst x64_bin_update_nth_error_other [of 6 l xpc u8_list l1 "xpc1+4" i2]; simp?; linarith?)
+              apply (subst x64_bin_update_nth_error_other [of 6 l xpc u8_list l1 "xpc1+5" i3]; simp?; linarith?)
+              apply (subst x64_bin_update_nth_error_other [of 6 l xpc u8_list l1 "xpc1+6" i4]; simp?; linarith?)
+              done
+
+            apply ((erule case_option_eq_NE; simp?) | (erule ifE; erule conjE; simp))+
+            subgoal for dst i1 i2 i3 i4 imm
+              apply (subst x64_bin_update_nth_error_other [of 6 l xpc u8_list l1 xpc1 h]; simp?; linarith?)
+              apply (subst x64_bin_update_nth_error_other [of 6 l xpc u8_list l1 "xpc1+1" op]; simp?; linarith?)
+              apply (subst x64_bin_update_nth_error_other [of 6 l xpc u8_list l1 "xpc1+2" reg]; simp?; linarith?)
+              apply (subst x64_bin_update_nth_error_other [of 6 l xpc u8_list l1 "xpc1+3" i1]; simp?; linarith?)
+              apply (subst x64_bin_update_nth_error_other [of 6 l xpc u8_list l1 "xpc1+4" i2]; simp?; linarith?)
+              apply (subst x64_bin_update_nth_error_other [of 6 l xpc u8_list l1 "xpc1+5" i3]; simp?; linarith?)
+              apply (subst x64_bin_update_nth_error_other [of 6 l xpc u8_list l1 "xpc1+6" i4]; simp?; linarith?)
+              done
+
+            apply ((erule case_option_eq_NE; simp?) | (erule ifE; erule conjE; simp))+
+            subgoal for dst i1 i2 i3 i4 imm
+              apply (subst x64_bin_update_nth_error_other [of 6 l xpc u8_list l1 xpc1 h]; simp?; linarith?)
+              apply (subst x64_bin_update_nth_error_other [of 6 l xpc u8_list l1 "xpc1+1" op]; simp?; linarith?)
+              apply (subst x64_bin_update_nth_error_other [of 6 l xpc u8_list l1 "xpc1+2" reg]; simp?; linarith?)
+              apply (subst x64_bin_update_nth_error_other [of 6 l xpc u8_list l1 "xpc1+3" i1]; simp?; linarith?)
+              apply (subst x64_bin_update_nth_error_other [of 6 l xpc u8_list l1 "xpc1+4" i2]; simp?; linarith?)
+              apply (subst x64_bin_update_nth_error_other [of 6 l xpc u8_list l1 "xpc1+5" i3]; simp?; linarith?)
+              apply (subst x64_bin_update_nth_error_other [of 6 l xpc u8_list l1 "xpc1+6" i4]; simp?; linarith?)
+              done
+
+            apply ((erule case_option_eq_NE; simp?) | (erule ifE; erule conjE; simp))+
+            subgoal for dst i1 i2 i3 i4 imm
+              apply (subst x64_bin_update_nth_error_other [of 6 l xpc u8_list l1 xpc1 h]; simp?; linarith?)
+              apply (subst x64_bin_update_nth_error_other [of 6 l xpc u8_list l1 "xpc1+1" op]; simp?; linarith?)
+              apply (subst x64_bin_update_nth_error_other [of 6 l xpc u8_list l1 "xpc1+2" reg]; simp?; linarith?)
+              apply (subst x64_bin_update_nth_error_other [of 6 l xpc u8_list l1 "xpc1+3" i1]; simp?; linarith?)
+              apply (subst x64_bin_update_nth_error_other [of 6 l xpc u8_list l1 "xpc1+4" i2]; simp?; linarith?)
+              apply (subst x64_bin_update_nth_error_other [of 6 l xpc u8_list l1 "xpc1+5" i3]; simp?; linarith?)
+              apply (subst x64_bin_update_nth_error_other [of 6 l xpc u8_list l1 "xpc1+6" i4]; simp?; linarith?)
+              done
+
+            subgoal
+              apply ((erule case_option_eq_NE; simp?) | (erule ifE; erule conjE; simp))+
+              subgoal for sib d1 d2 d3 d4 dis
+                apply (erule conjE)
+                apply ((erule case_option_eq_NE; simp?) | (erule ifE; erule conjE; simp))+
+                done
+              done
+
+            apply ((erule case_option_eq_NE; simp?) | (erule ifE; erule conjE; simp))+
+            subgoal for imm dst
+              apply (subst x64_bin_update_nth_error_other [of 6 l xpc u8_list l1 xpc1 h]; simp?; linarith?)
+              apply (subst x64_bin_update_nth_error_other [of 6 l xpc u8_list l1 "xpc1+1" op]; simp?; linarith?)
+              apply (subst x64_bin_update_nth_error_other [of 6 l xpc u8_list l1 "xpc1+2" reg]; simp?; linarith?)
+              apply (subst x64_bin_update_nth_error_other [of 6 l xpc u8_list l1 "xpc1+3" imm]; simp?; linarith?)
+              done
+            subgoal for imm
+              apply ((erule case_option_eq_NE; simp?) | (erule ifE; erule conjE; simp))+
+              subgoal for dst
+                apply (subst x64_bin_update_nth_error_other [of 6 l xpc u8_list l1 xpc1 h]; simp?; linarith?)
+                apply (subst x64_bin_update_nth_error_other [of 6 l xpc u8_list l1 "xpc1+1" op]; simp?; linarith?)
+                apply (subst x64_bin_update_nth_error_other [of 6 l xpc u8_list l1 "xpc1+2" reg]; simp?; linarith?)
+                apply (subst x64_bin_update_nth_error_other [of 6 l xpc u8_list l1 "xpc1+3" imm]; simp?; linarith?)
+                done
+              apply ((erule case_option_eq_NE; simp?) | (erule ifE; erule conjE; simp))+
+              subgoal for dst
+                apply (subst x64_bin_update_nth_error_other [of 6 l xpc u8_list l1 xpc1 h]; simp?; linarith?)
+                apply (subst x64_bin_update_nth_error_other [of 6 l xpc u8_list l1 "xpc1+1" op]; simp?; linarith?)
+                apply (subst x64_bin_update_nth_error_other [of 6 l xpc u8_list l1 "xpc1+2" reg]; simp?; linarith?)
+                apply (subst x64_bin_update_nth_error_other [of 6 l xpc u8_list l1 "xpc1+3" imm]; simp?; linarith?)
+                done
+              done
+
+            apply ((erule case_option_eq_NE; simp?) | (erule ifE; erule conjE; simp))+
+            subgoal for dis src dst
+              apply (subst x64_bin_update_nth_error_other [of 6 l xpc u8_list l1 xpc1 h]; simp?; linarith?)
+              apply (subst x64_bin_update_nth_error_other [of 6 l xpc u8_list l1 "xpc1+1" op]; simp?; linarith?)
+              apply (subst x64_bin_update_nth_error_other [of 6 l xpc u8_list l1 "xpc1+2" reg]; simp?; linarith?)
+              apply (subst x64_bin_update_nth_error_other [of 6 l xpc u8_list l1 "xpc1+3" dis]; simp?; linarith?)
+              done
+            apply ((erule case_option_eq_NE; simp?) | (erule ifE; erule conjE; simp))+
+            subgoal for dis src dst
+              apply (subst x64_bin_update_nth_error_other [of 6 l xpc u8_list l1 xpc1 h]; simp?; linarith?)
+              apply (subst x64_bin_update_nth_error_other [of 6 l xpc u8_list l1 "xpc1+1" op]; simp?; linarith?)
+              apply (subst x64_bin_update_nth_error_other [of 6 l xpc u8_list l1 "xpc1+2" reg]; simp?; linarith?)
+              apply (subst x64_bin_update_nth_error_other [of 6 l xpc u8_list l1 "xpc1+3" dis]; simp?; linarith?)
+              done
+            subgoal
+              apply ((erule case_option_eq_NE; simp?) | (erule ifE; erule conjE; simp))+
+              subgoal for d1 d2 d3 d4 dis src dst
+                apply (subst x64_bin_update_nth_error_other [of 6 l xpc u8_list l1 xpc1 h]; simp?; linarith?)
+                apply (subst x64_bin_update_nth_error_other [of 6 l xpc u8_list l1 "xpc1+1" op]; simp?; linarith?)
+                apply (subst x64_bin_update_nth_error_other [of 6 l xpc u8_list l1 "xpc1+2" reg]; simp?; linarith?)
+                apply (erule conjE)
+                apply (subst x64_bin_update_nth_error_other [of 6 l xpc u8_list l1 "xpc1+3" d1]; simp?; linarith?)
+                apply (subst x64_bin_update_nth_error_other [of 6 l xpc u8_list l1 "xpc1+4" d2]; simp?; linarith?)
+                apply (subst x64_bin_update_nth_error_other [of 6 l xpc u8_list l1 "xpc1+5" d3]; simp?; linarith?)
+                apply (subst x64_bin_update_nth_error_other [of 6 l xpc u8_list l1 "xpc1+6" d4]; simp?; linarith?)
+                done
+              apply ((erule case_option_eq_NE; simp?) | (erule ifE; erule conjE; simp))+
+              done
+            apply ((erule case_option_eq_NE; simp?) | (erule ifE; erule conjE; simp))+
+            done
+          done
+        done
+      done
+    done
+  done
 
 end
